updated to ref flag

theories/typechecker/typechecker.v
@@ -78,7 +78,7 @@ Proof.
   by apply check_ok_true_to_prop.
 Qed.
 
-(* A few tactics *)
+(** TACTICS **)
 Ltac solve_Forall_foldr HForall Hfoldr checker proper :=
   apply (Forall_impl _ (λ x, check_ok checker x = true -> proper x)) in HForall;
   [ eapply Forall_foldr_bool_to_prop; [apply HForall | apply Hfoldr] |
@@ -88,8 +88,316 @@ Ltac solve_Forall_foldr HForall Hfoldr checker proper :=
 Ltac destruct_on_if_equal resname :=
   match goal with
     | H:((if ?key then _ else _)=_) |- _ => destruct key eqn:resname
+  end.
+
+Ltac stupid_unit o :=
+  unfold ok in o; assert (HO: o = tt) by (by destruct o); subst.
+
+
+Ltac structural_auto :=
+   match goal with
+  | H: (_ && _ = true) |- _ => apply andb_prop in H; destruct H as [?H1 ?H2]
+  | o:ok |- _ => stupid_unit o
+  | H: ok_term = ok_term |- _ => clear H
+  | H: (andb _ _ = true) |- _ => apply andb_prop in H; destruct H as [?H1 ?H2]
+  | H: true = false |- _ => inversion H
+  | H: false = true |- _ => inversion H
+  | H: ((match ?key with |_=>_ end) = _) |- _ => destruct key eqn:?HMatch; try inversion H; simpl in *
+  | H:((if ?key then _ else _)=_) |- _ => destruct key eqn:?HMatch; try (inversion H; [idtac]; clear H); simpl in *
+   end.
+
+
+
+
+(** BOOLEAN EQUALITIES **)
+(*
+Scheme Equality for copyability.
+Scheme Equality for dropability.*)
+Scheme Equality for ref_flag.
+Scheme Equality for atomic_rep.
+Scheme Equality for base_memory.
+Scheme Equality for memory.
+Scheme Equality for list.
+Scheme Equality for num_type.
+Scheme Equality for primitive.
+
+(*
+Lemma copyability_eq_convert :
+  ∀ c1 c2, copyability_beq c1 c2 = true <-> c1 = c2.
+Proof.
+  split; intros;
+    [by apply internal_copyability_dec_bl in H | by apply internal_copyability_dec_lb in H].
+Qed.
+Lemma dropability_eq_convert :
+  ∀ d1 d2, dropability_beq d1 d2 = true <-> d1 = d2.
+Proof.
+  split; intros;
+   [by apply internal_dropability_dec_bl in H | by apply internal_dropability_dec_lb in H].
+Qed.
+*)
+Lemma ref_flag_eq_convert :
+  ∀ ξ1 ξ2, ref_flag_beq ξ1 ξ2 = true <-> ξ1 = ξ2.
+Proof.
+  split; intros;
+    [by apply internal_ref_flag_dec_bl in H | by apply internal_ref_flag_dec_lb in H].
+Qed.
+
+Fixpoint representation_beq (r1:representation) (r2:representation) : bool :=
+  match r1, r2 with
+  | VarR i1, VarR i2 => (i1 =? i2)
+  | SumR r1s, SumR r2s => list_beq representation representation_beq r1s r2s
+  | ProdR r1s, ProdR r2s => list_beq representation representation_beq r1s r2s
+  | AtomR a1, AtomR a2 => atomic_rep_beq a1 a2
+  | _, _ => false
+  end.
+
+Lemma representation_eq_convert_forward :
+  ∀ r1, (∀ r2, representation_beq r1 r2 = true -> r1 = r2).
+Proof.
+  induction r1 using rep_ind.
+  * intros; destruct r2; simpl in H; try inversion H. apply Nat.eqb_eq in H; by subst.
+  * intros. destruct r2; simpl in H0; try inversion H0. clear H2.
+    pose proof internal_list_dec_bl as ToUse.
+    specialize (ToUse representation representation_beq).
+
+    (* I'm confused actually. To use internal_list_dec_bl, I need to
+       have a proof of representation_beq r1 r2 = true -> r1 = r2, but the
+       IH is specific to ρs.
+       TODO *)
+Admitted.
+
+Lemma representation_eq_convert_backward :
+  ∀ r1 r2, r1 = r2 -> representation_beq r1 r2 = true.
+Proof.
+  intros; subst.
+  induction r2 using rep_ind.
+  * simpl. apply Nat.eqb_refl.
+  * simpl.
+    (* Hm once again a similar issue. *)
+Admitted.
+
+Lemma representation_eq_convert :
+  ∀ r1 r2, representation_beq r1 r2 = true <-> r1 = r2.
+Proof.
+  split; [apply representation_eq_convert_forward | apply representation_eq_convert_backward].
+Qed.
+
+Fixpoint size_beq (s1:size) (s2:size) : bool :=
+  match s1, s2 with
+  | VarS i1, VarS i2 => (i1 =? i2)
+  | SumS s1s, SumS s2s => list_beq size size_beq s1s s2s
+  | ProdS s1s, ProdS s2s => list_beq size size_beq s1s s2s
+  | RepS r1, RepS r2 => representation_beq r1 r2
+  | ConstS n1, ConstS n2 => (n1 =? n2)
+  | _, _ => false
+  end.
+
+Lemma size_eq_convert :
+  ∀ s1 s2, size_beq s1 s2 = true <-> s1 = s2.
+Proof.
+  (* Same issue happens here *)
+Admitted.
+
+Fixpoint kind_beq (k1:kind) (k2:kind) : bool :=
+  match k1, k2 with
+  | VALTYPE r1 ξ1, VALTYPE r2 ξ2 =>
+      andb (representation_beq r1 r2) (ref_flag_beq ξ1 ξ2)
+  | MEMTYPE s1 ξ1, MEMTYPE s2 ξ2 =>
+      andb (size_beq s1 s2) (ref_flag_beq ξ1 ξ2)
+  | _, _ => false
+  end.
+
+Lemma kind_eq_convert :
+  ∀ k1 k2, kind_beq k1 k2 = true <-> k1 = k2.
+Proof.
+  split.
+  (* fix to deal with ref flag
+  - intros. destruct k1, k2; simpl in H; try inversion H; clear H1; repeat structural_auto.
+    * apply representation_eq_convert in H1.
+      apply copyability_eq_convert in H0.
+      apply internal_dropability_dec_bl in H2. subst; auto.
+    * apply size_eq_convert in H1.
+      apply internal_dropability_dec_bl in H2. subst; auto.
+  - intros; subst. destruct k2; simpl.
+    * apply andb_true_intro; split; [|apply andb_true_intro; split].
+      + assert (H:r=r) by auto. apply representation_eq_convert in H. auto.
+      + assert (H:c=c) by auto. apply copyability_eq_convert in H; auto.
+      + assert (H:d=d) by auto. apply internal_dropability_dec_lb in H. auto.
+    * apply andb_true_intro; split.
+      + assert (H:s=s) by auto. apply size_eq_convert in H; auto.
+      + assert (H:d=d) by auto. apply internal_dropability_dec_lb in H; auto.
+*)
+Admitted.
+
+Lemma kind_neq_convert :
+  ∀ k1 k2, kind_beq k1 k2 = false <-> k1 <> k2.
+Proof.
+  split; intros.
+  (* there's some decidability lemmas that would need to be done. This is fine to leave. *)
+Admitted.
+
+
+Lemma num_type_eq_convert :
+  ∀ nt1 nt2, num_type_beq nt1 nt2 = true <-> nt1 = nt2.
+Proof.
+  split; intros;
+    [by apply internal_num_type_dec_bl in H | by apply internal_num_type_dec_lb in H].
+Admitted.
+
+(* type beq. Oh boy. Let's go. *)
+Fixpoint type_beq (τ1:type) (τ2:type) : bool :=
+  match τ1, τ2 with
+  | VarT i1, VarT i2 => i1 =? i2
+  | I31T κ1, I31T κ2 => kind_beq κ1 κ2
+  | NumT κ1 nt1, NumT κ2 nt2 => andb (kind_beq κ1 κ2) (num_type_beq nt1 nt2)
+  | SumT κ1 τs1, SumT κ2 τs2
+  | VariantT κ1 τs1, VariantT κ2 τs2
+  | ProdT κ1 τs1, ProdT κ2 τs2
+  | StructT κ1 τs1, StructT κ2 τs2 =>
+      andb (kind_beq κ1 κ2) (list_beq type type_beq τs1 τs2)
+  | RefT κ1 m1 τ1, RefT κ2 m2 τ2 =>
+      andb (andb (kind_beq κ1 κ2) (memory_beq m1 m2)) (type_beq τ1 τ2)
+  | CodeRefT κ1 ft1, CodeRefT κ2 ft2 =>
+      andb (kind_beq κ1 κ2) (function_type_beq ft1 ft2)
+  | SerT κ1 t1, SerT κ2 t2 => andb (kind_beq κ1 κ2) (type_beq t1 t2)
+  | PlugT κ1 ρ1, PlugT κ2 ρ2 => andb (kind_beq κ1 κ2) (representation_beq ρ1 ρ2)
+  | SpanT κ1 σ1, SpanT κ2 σ2 => andb (kind_beq κ1 κ2) (size_beq σ1 σ2)
+  | RecT κ1 t1, RecT κ2 t2
+  | ExistsMemT κ1 t1, ExistsMemT κ2 t2
+  | ExistsRepT κ1 t1, ExistsRepT κ2 t2
+  | ExistsSizeT κ1 t1, ExistsSizeT κ2 t2 =>
+      andb (kind_beq κ1 κ2) (type_beq t1 t2)
+  | ExistsTypeT κ11 κ12 t1, ExistsTypeT κ21 κ22 t2 =>
+      andb (andb (kind_beq κ11 κ21) (kind_beq κ12 κ22)) (type_beq t1 t2)
+  | _, _ => false
   end
-.
+with function_type_beq (fτ1:function_type) (fτ2:function_type) : bool :=
+  match fτ1, fτ2 with
+  | MonoFunT τs11 τs12, MonoFunT τs21 τs22 =>
+      andb (list_beq type type_beq τs11 τs21) (list_beq type type_beq τs12 τs22)
+  | ForallMemT ft1, ForallMemT ft2
+  | ForallRepT ft1, ForallRepT ft2
+  | ForallSizeT ft1, ForallSizeT ft2 => function_type_beq ft1 ft2
+  | ForallTypeT κ1 ft1, ForallTypeT κ2 ft2 =>
+      andb (kind_beq κ1 κ2) (function_type_beq ft1 ft2)
+  | _, _ => false
+  end.
+
+
+
+
+
+(* I should prove these eventually. Mainly to convince myself that
+list_beq will do what I want it to do. Although I think it's just fine.
+
+ TODO *)
+Lemma type_eq_convert :
+  ∀ τ1 τ2, type_beq τ1 τ2 = true <-> τ1 = τ2.
+Proof. Admitted.
+
+Lemma function_type_eq_convert :
+  ∀ ft1 ft2, function_type_beq ft1 ft2 = true <-> ft1 = ft2.
+Proof. Admitted.
+
+
+Lemma memory_eq_convert :
+  ∀ m1 m2, memory_beq m1 m2 = true <-> m1 = m2.
+Proof.
+   split; intros;
+    [by apply internal_memory_dec_bl in H | by apply internal_memory_dec_lb in H].
+Qed.
+
+(* I'm bad at everything so monomorphic *)
+Lemma list_eq_convert_type :
+  ∀ τs1 τs2, list_beq type type_beq τs1 τs2 = true <-> τs1 = τs2.
+Proof. Admitted.
+Lemma list_eq_convert_size :
+  ∀ τs1 τs2, list_beq size size_beq τs1 τs2 = true <-> τs1 = τs2.
+Proof. Admitted.
+Definition local_ctx_beq (L L':local_ctx) : bool := list_beq type type_beq L L'.
+Lemma local_ctx_eq_convert :
+  ∀ L L', local_ctx_beq L L' = true <-> L = L'.
+Proof.
+  split; intros; unfold local_ctx_beq in *.
+  - apply list_eq_convert_type in H; subst; auto.
+  - subst; apply list_eq_convert_type; auto.
+Qed.
+Definition module_type_beq (m1:module_type) (m2:module_type) : bool :=
+  andb (list_beq function_type function_type_beq m1.(mt_imports) m2.(mt_imports))
+       (list_beq function_type function_type_beq m1.(mt_exports) m2.(mt_exports)).
+Lemma module_type_eq_convert :
+  ∀ m1 m2, module_type_beq m1 m2 = true <-> m1 = m2.
+Proof.
+  split; intros.
+  - destruct m1, m2.
+    unfold module_type_beq in H.
+    (* yup the things that are equal are equal *)
+    admit.
+  - subst.
+    destruct m2.
+    unfold module_type_beq. cbn.
+    (* yup it's equal *)
+    admit.
+    (* to complete this, it's a list_beq thing *)
+Admitted.
+Definition instruction_type_beq (inst1 inst2:instruction_type) : bool :=
+  match inst1, inst2 with
+  | InstrT τs11 τs12, InstrT τs21 τs22 =>
+      andb (list_beq type type_beq τs11 τs21) (list_beq type type_beq τs12 τs22)
+  end.
+Lemma instruction_type_eq_convert :
+  ∀ inst1 inst2, instruction_type_beq inst1 inst2 = true <-> inst1 = inst2.
+Proof.
+  split; intros; destruct inst1, inst2; unfold instruction_type_beq in *; simpl in *.
+  - repeat structural_auto. apply list_eq_convert_type in H1, H2. subst; auto.
+  - inversion H; subst.
+    apply andb_true_intro; split; apply list_eq_convert_type; auto.
+Qed.
+Definition path_result_beq (pres1 pres2:path_result) : bool :=
+  andb (andb (list_beq type type_beq pres1.(pr_prefix) pres2.(pr_prefix))
+             (type_beq pres1.(pr_target) pres2.(pr_target)))
+             (type_beq pres1.(pr_replaced) pres2.(pr_replaced)).
+
+Lemma path_result_eq_convert :
+  ∀ pres1 pres2, path_result_beq pres1 pres2 = true <-> pres1 = pres2.
+Proof.
+  split; intros.
+  - unfold path_result_beq in H.
+    repeat structural_auto.
+    apply list_eq_convert_type in H1.
+    apply type_eq_convert in H0, H2.
+    destruct pres1, pres2.
+    simpl in *. subst.
+    auto.
+  - destruct pres1, pres2.
+    inversion H; subst.
+    unfold path_result_beq. simpl.
+    apply andb_true_intro. split; [apply andb_true_intro; split |].
+    + apply list_eq_convert_type. auto.
+    + apply type_eq_convert; auto.
+    + apply type_eq_convert; auto.
+Qed.
+
+
+Ltac boolean_equality_auto :=
+  match goal with
+  | H: (kind_beq _ _ = true) |- _ => apply kind_eq_convert in H; subst; auto
+  | H: (instruction_type_beq _ _ = true) |- _ => apply instruction_type_eq_convert in H; subst; auto
+  | H: (local_ctx_beq _ _ = true) |- _ => apply local_ctx_eq_convert in H; subst; auto
+  | H: (representation_beq _ _ = true) |- _ => apply representation_eq_convert in H; subst; auto
+  | H: (ref_flag_beq _ _ = true) |- _ => apply ref_flag_eq_convert in H; subst; auto
+  | H: (size_beq _ _ = true) |- _ => apply size_eq_convert in H; subst; auto
+  | H: (function_type_beq _ _ = true) |- _ => apply function_type_eq_convert in H; subst; auto
+  | H: (type_beq _ _ = true) |- _ => apply type_eq_convert in H; subst; auto
+  | H: (instruction_type_beq _ _ = true) |- _ => apply instruction_type_eq_convert in H; subst; auto
+  | H: (module_type_beq _ _ = true) |- _ => apply module_type_eq_convert in H; subst; auto
+  | H: (memory_beq _ _ = true) |- _ => apply memory_eq_convert in H; subst; auto
+  | H: (num_type_beq _ _ = true) |- _ => apply num_type_eq_convert in H; subst; auto
+  | H: (path_result_beq _ _ = true) |- _ => apply path_result_eq_convert in H; subst; auto
+  | H: (list_beq type type_beq _ _ = true) |- _ => apply list_eq_convert_type in H; subst; auto
+  | H: (list_beq size size_beq _ _ = true) |- _ => apply list_eq_convert_size in H; subst; auto
+  end.
+
 
 
 
@@ -153,12 +461,7 @@ Fixpoint size_ok_checker (k:kind_ctx) (s:size) : type_checker_res :=
   match s with
   | ConstS n => ok_term
   | VarS r => if r <? k.(kc_size_vars) then ok_term else INR "size_ok error"
-  | RepS ρ => match (rep_ok_checker k ρ) with
-              | inl _ => ok_term
-              | err => err (* this allows propagation*)
-                         (* you could also just ret rep_ok_checker. Idk which would be
-                          better for future changeability. I'll do just ret later*)
-              end
+  | RepS ρ => rep_ok_checker k ρ
   | SumS σs =>
       if (foldr (λ i:size, andb (check_ok (size_ok_checker k) i)) true σs)
            then ok_term else INR "size_ok error"
@@ -171,21 +474,13 @@ Lemma size_ok_checker_correct (k:kind_ctx) (s:size) :
   (size_ok_checker k s = ok_term) -> size_ok k s.
 Proof.
   intros.
-  induction s using size_ind; simpl in H.
-  - apply OKVarS.
-    destruct_on_if_equal H'; [apply Nat.ltb_lt in H'; auto | inversion H].
+  induction s using size_ind; simpl in H; repeat structural_auto.
+  - apply Nat.ltb_lt in HMatch; auto; by constructor.
   - apply OKSumS.
-    destruct_on_if_equal Hfoldr; [solve_Forall_foldr H0 Hfoldr (size_ok_checker k) (size_ok k) | inversion H].
+    solve_Forall_foldr H0 HMatch (size_ok_checker k) (size_ok k).
   - apply OKProdS.
-    destruct_on_if_equal Hfoldr; [solve_Forall_foldr H0 Hfoldr (size_ok_checker k) (size_ok k) | inversion H].
-  - apply OKRepS.
-    simpl in H.
-    destruct (rep_ok_checker k ρ) eqn:H'.
-    + apply rep_ok_checker_correct.
-      unfold ok in o.
-      assert (o = tt) by (by destruct o).
-      subst; auto.
-    + inversion H.
+    solve_Forall_foldr H0 HMatch (size_ok_checker k) (size_ok k).
+  - apply OKRepS. apply rep_ok_checker_correct in H; auto.
   - apply OKConstS.
 Qed.
 
@@ -193,8 +488,8 @@ Qed.
 (* kind_ok *)
 Definition kind_ok_checker (k:kind_ctx) (ki: kind) : type_checker_res :=
   match ki with
-  | (VALTYPE ρ χ δ) => rep_ok_checker k ρ
-  | MEMTYPE σ δ => size_ok_checker k σ
+  | (VALTYPE ρ ξ) => rep_ok_checker k ρ
+  | MEMTYPE σ ξ => size_ok_checker k σ
   end.
 
 Lemma kind_ok_checker_correct (k:kind_ctx) (ki:kind) :
@@ -312,17 +607,13 @@ Ltac destruct_on_match_equal resname :=
   | H: ((match ?key with |_=>_ end) = _) |- _ => destruct key eqn:resname
   end.
 
-Ltac stupid_unit o :=
-  unfold ok in o; assert (HO: o = tt) by (by destruct o); subst.
 
 Ltac destruct_match_unit Hmatch resname o :=
   destruct_on_match_equal resname; [stupid_unit o | inversion Hmatch].
 
 Ltac my_auto :=
-  match goal with
-  | H: ((match ?key with |_=>_ end) = _) |- _ => destruct key eqn:?HMatch; [ | inversion H ]
-  | H:((if ?key then _ else _)=_) |- _ => destruct key eqn:?HMatch; [ | inversion H ]
-  | o:ok |- _ => stupid_unit o
+  try structural_auto; try boolean_equality_auto;
+  try match goal with
   | H: (kind_ok_checker _ _ = inl ()) |- _ => apply kind_ok_checker_correct in H; auto
   | H: (kind_ok_checker _ _ = ok_term) |- _ => apply kind_ok_checker_correct in H; auto
   | H: (mem_ok_checker _ _ = inl ()) |- _ => apply mem_ok_checker_correct in H; auto
@@ -339,7 +630,7 @@ Ltac find_Forall_foldr checker prop :=
       solve_Forall_foldr HForall Hfoldr checker prop
   end.
 
-Lemma type_ok_checker_correct :
+Lemma type_ok_checker_correct_basic :
   (forall t F, (type_ok_checker F t = ok_term) -> type_ok F t) /\
   (forall ft F, function_type_ok_checker F ft = ok_term -> function_type_ok F ft).
 Proof.
@@ -360,12 +651,2764 @@ Proof.
 
 Qed.
 
+Lemma type_ok_checker_correct :
+  ∀ t F, (type_ok_checker F t = ok_term) -> type_ok F t.
+Proof.
+  apply type_ok_checker_correct_basic.
+Qed.
 
-(* Have to define an equality operator on representation and dropability *)
-Fixpoint subkind_of_checker (κ1:kind) (κ2:kind) : type_checker_res :=
+Lemma function_type_ok_checker_correct :
+  ∀ ft F, function_type_ok_checker F ft = ok_term -> function_type_ok F ft.
+Proof.
+  apply type_ok_checker_correct_basic.
+Qed.
+
+
+
+Definition mono_mem_checker (μ:memory) : type_checker_res :=
+  match μ with
+  | BaseM bm => ok_term
+  | _ => INR "not monomem"
+  end.
+
+Definition subkind_of_checker (κ1:kind) (κ2:kind) : type_checker_res :=
   match κ1, κ2 with
-  | (VALTYPE ρ1 ImCopy δ1), (VALTYPE ρ2 ExCopy δ2) =>
-      (* this true here is fake *)
-      if true then ok_term else INR "not subkind"
+  | (VALTYPE ρ1 NoRefs), (VALTYPE ρ2 GCRefs) =>
+      if (representation_beq ρ1 ρ2)
+      then ok_term else INR "fail in subkind check"
+  | (VALTYPE ρ1 GCRefs), (VALTYPE ρ2 AnyRefs) =>
+      if (representation_beq ρ1 ρ2)
+      then ok_term else INR "fail in subkind check"
+  | (MEMTYPE σ1 NoRefs), (MEMTYPE σ2 GCRefs) =>
+      if size_beq σ1 σ2
+      then ok_term else INR "fail in subkind check"
+  | (MEMTYPE σ1 GCRefs), (MEMTYPE σ2 AnyRefs) =>
+      if size_beq σ1 σ2
+      then ok_term else INR "fail in subkind check"
   | _, _ => INR "no"
   end.
+
+
+
+
+Ltac my_auto2 :=
+  try structural_auto; try boolean_equality_auto;
+  try match goal with
+  | H: (kind_ok_checker _ _ = inl ()) |- _ => apply kind_ok_checker_correct in H; auto
+  | H: (kind_ok_checker _ _ = ok_term) |- _ => apply kind_ok_checker_correct in H; auto
+  | H: (mem_ok_checker _ _ = inl ()) |- _ => apply mem_ok_checker_correct in H; auto
+  | H: (mem_ok_checker _ _ = ok_term) |- _ => apply mem_ok_checker_correct in H; auto
+  | H: (rep_ok_checker _ _ = inl ()) |- _ => apply rep_ok_checker_correct in H; auto
+  | H: (rep_ok_checker _ _ = ok_term) |- _ => apply rep_ok_checker_correct in H; auto
+  | H: (size_ok_checker _ _ = inl ()) |- _ => apply size_ok_checker_correct in H; auto
+  | H: (size_ok_checker _ _ = ok_term) |- _ => apply size_ok_checker_correct in H; auto
+  | H: (type_ok_checker _ _ = inl ()) |- _ => apply type_ok_checker_correct in H; auto
+  | H: (type_ok_checker _ _ = ok_term) |- _ => apply type_ok_checker_correct in H; auto
+  | H: (function_type_ok_checker _ _ = inl ()) |- _ => apply function_type_ok_checker_correct in H; auto
+  | H: (function_type_ok_checker _ _ = ok_term) |- _ => apply function_type_ok_checker_correct in H; auto
+end.
+
+
+Lemma subkind_of_checker_correct :
+  ∀ k1 k2, subkind_of_checker k1 k2 = ok_term -> subkind_of k1 k2.
+Proof.
+  intros.
+  destruct k1, k2.
+  2, 3: cbn in H; repeat structural_auto.
+  2: destruct r, r0. 1: destruct r0, r2.
+  all: simpl in H; try inversion H; repeat my_auto2; constructor.
+Qed.
+
+Definition has_kind_ok_checker (F:function_ctx) (t:type) (k:kind) : type_checker_res :=
+  match (type_ok_checker F t) with
+  | inl () => (kind_ok_checker (F.(fc_kind_ctx)) k)
+  | err => err
+  end.
+
+Lemma has_kind_ok_checker_correct :
+  ∀ F t k, has_kind_ok_checker F t k = ok_term -> has_kind_ok F t k.
+Proof.
+  intros. unfold has_kind_ok_checker in H. repeat my_auto2.
+  constructor; auto.
+Qed.
+
+
+
+
+
+(* This function just grabs the kind out of the type *)
+Definition grab_kind (F:function_ctx) (t:type) : option kind :=
+  type_kind (F.(fc_type_vars)) t.
+
+
+
+(* A thing that helps with subkinding *)
+Definition check_if_subkind (k1:kind) (k2:kind) : type_checker_res :=
+  match k1, k2 with
+  | VALTYPE ρ1 ξ1, VALTYPE ρ2 ξ2 =>
+      if representation_beq ρ1 ρ2
+      then
+        match ξ1, ξ2 with
+        | NoRefs, _
+        | GCRefs, GCRefs
+        | GCRefs, AnyRefs
+        | AnyRefs, AnyRefs => ok_term
+        | _, _ => INR "not subkind"
+        end
+      else INR "mismatch in representation for subkinds"
+  | MEMTYPE σ1 ξ1, MEMTYPE σ2 ξ2 =>
+      if size_beq σ1 σ2
+      then
+        match ξ1, ξ2 with
+        | NoRefs, _
+        | GCRefs, GCRefs
+        | GCRefs, AnyRefs
+        | AnyRefs, AnyRefs => ok_term
+        | _, _ => INR "not subkind"
+        end
+      else INR "mismatch in sizity for subkinds"
+  | _, _ => INR "mismatch in general kind for subkind"
+  end.
+
+Lemma check_if_subkind_works_with_has_kind :
+  ∀ F τ k1 k2,
+    check_if_subkind k1 k2 = ok_term ->
+    has_kind F τ k1 ->
+    has_kind F τ k2.
+Proof.
+  Ltac local_auto := eapply KSub; try constructor; auto.
+  
+  intros.
+  destruct k1, k2; simpl in H; repeat my_auto2; subst; auto; try (inversion H).
+  - destruct r2; auto; local_auto. local_auto.
+  - local_auto.
+  - destruct r0; auto; local_auto. local_auto.
+  - local_auto.
+Qed.
+
+
+
+Fixpoint foldr2 {A B C : Type} (f : B → C → A → A) (a0 : A)
+  (lB : list B) (lC : list C) :=
+  match lB, lC with
+  | b :: lB0, c :: lC0 => f b c (foldr2 f a0 lB0 lC0)
+  | _, _ => a0
+  end.
+
+
+(* Check kind in a naive way. I guess. *)
+Fixpoint has_kind_checker (F:function_ctx) (t:type) (k:kind) : type_checker_res :=
+  match t with
+  | VarT t =>
+      match (F.(fc_type_vars)) !! t with
+      | Some κ =>
+          match kind_ok_checker (F.(fc_kind_ctx)) κ with
+          | inl () => check_if_subkind κ k
+          | err => err
+          end
+      | None => INR "variable not in there or smthn"
+      end
+  (* Numbers *)
+  | I31T κ =>
+      if (kind_beq κ (VALTYPE (AtomR PtrR) NoRefs))
+      then check_if_subkind κ k
+      else INR "wrong kind for I31T"
+    (* NumT *)
+  | NumT κ (IntT I32T) =>
+      if (kind_beq κ (VALTYPE (AtomR I32R) NoRefs))
+      then check_if_subkind κ k
+      else INR "wrong kind for I32T"
+  | NumT κ (IntT I64T) =>
+      if (kind_beq κ (VALTYPE (AtomR I64R) NoRefs) )
+      then check_if_subkind κ k
+      else INR "wrong kind for I64T"
+  | NumT κ (FloatT F32T) =>
+      if (kind_beq κ (VALTYPE (AtomR F32R) NoRefs))
+      then check_if_subkind κ k
+      else INR "wrong kind for F32T"
+  | NumT κ (FloatT F64T) =>
+      if (kind_beq κ (VALTYPE (AtomR F64R) NoRefs))
+      then check_if_subkind κ k
+      else INR "wrong kind for F64T"
+  (* Sums and Prods *)
+  | SumT κ τs =>
+      match κ with
+      | VALTYPE (SumR ρs) ξ =>
+          if foldr2
+               (λ t:type, λ r:representation,
+                  andb (check_ok_output (has_kind_checker F t (VALTYPE r ξ)))
+               ) true τs ρs
+          then check_if_subkind κ k
+          else INR "bad sum kind internals"
+      | _ => INR "bad sum kind format"
+      end
+  | VariantT κ τs =>
+      match κ with
+      | MEMTYPE (SumS σs) ξ =>
+          if foldr2
+               (λ t:type, λ s:size,
+                  andb (check_ok_output (has_kind_checker F t (MEMTYPE s ξ)))
+               ) true τs σs
+          then check_if_subkind κ k
+          else INR "bad sum kind internals"
+      | _ => INR "bad variant kind format"
+      end
+   | ProdT κ τs =>
+      match κ with
+      | VALTYPE (ProdR ρs) ξ =>
+          if foldr2
+               (λ t:type, λ r:representation,
+                  andb (check_ok_output (has_kind_checker F t (VALTYPE r ξ)))
+               ) true τs ρs
+          then check_if_subkind κ k
+          else INR "bad sum kind internals"
+      | _ => INR "bad prod kind format"
+      end
+  | StructT κ τs =>
+      match κ with
+      | MEMTYPE (ProdS σs) ξ =>
+          if foldr2
+               (λ t:type, λ s:size,
+                  andb (check_ok_output (has_kind_checker F t (MEMTYPE s ξ)))
+               ) true τs σs
+          then check_if_subkind κ k
+          else INR "bad sum kind internals"
+      | _ => INR "bad struct kind format"
+      end
+  (* References *)
+  | RefT κ (BaseM MemGC) τ =>
+      if (kind_beq κ (VALTYPE (AtomR PtrR) GCRefs))
+      then
+        match grab_kind F τ with
+          | Some innerk =>
+              match innerk with
+              | MEMTYPE σ ξ =>
+                  match has_kind_checker F τ (MEMTYPE σ ξ) with
+                  | inl () => check_if_subkind κ k
+                  | err => err
+                  end
+              | _ => INR "you have a reft t where t isnt memtype"
+              end
+          | None => INR "i think you have a bad variable or smthn"
+          end
+      else INR "bad gc mem kind format"
+  | RefT κ μ τ =>
+      if (kind_beq κ (VALTYPE (AtomR PtrR) AnyRefs))
+      then
+        match mem_ok_checker (F.(fc_kind_ctx)) μ with
+          | inl () =>
+              match grab_kind F τ with
+              | Some innerk =>
+                  match innerk with
+                  | MEMTYPE σ ξ =>
+                      match has_kind_checker F τ (MEMTYPE σ ξ) with
+                      | inl () => check_if_subkind κ k
+                      | err => err
+                      end
+                  | _ => INR "you have ref t where t isnt memtype"
+                  end
+              | None => INR "i think you have a bad variable or smthn"
+              end
+          | err => err
+          end
+      else INR "bad ref kind format"
+  | CodeRefT κ ϕ =>
+      match κ with
+      | VALTYPE (AtomR I32R) NoRefs =>
+          match function_type_ok_checker F ϕ with
+          | inl () => check_if_subkind κ k
+          | err => err
+          end
+      | _ => INR "bad coderef kind format"
+      end
+  (* Some weird ones I guess *)
+  | SerT κ τ =>
+      match κ with
+      | MEMTYPE (RepS ρ) ξ =>
+          match has_kind_checker F τ (VALTYPE ρ ξ) with
+          | inl () => check_if_subkind κ k
+          | err => err
+          end
+      | _ => INR "bad ser kind format"
+      end
+  | PlugT κ ρ =>
+      match κ with
+      | VALTYPE ρ1 NoRefs =>
+          if representation_beq ρ ρ1
+          then
+            match rep_ok_checker (F.(fc_kind_ctx)) ρ with
+            | inl () => check_if_subkind κ k
+            | err => err
+            end
+          else INR "plug's rep doesn't match kind's rep"
+      | _ => INR "bad plug kind format"
+      end
+  | SpanT κ σ =>
+      match κ with
+      | MEMTYPE σ1 NoRefs =>
+          if size_beq σ σ1
+          then
+            match size_ok_checker (F.(fc_kind_ctx)) σ with
+            | inl () => check_if_subkind κ k
+            | err => err
+            end
+          else INR "span's size doesn't match kind's size"
+      | _ => INR "bad span kind format"
+      end
+  | RecT κ τ =>
+      match has_kind_checker (F <| fc_type_vars ::= cons κ |>) τ κ with
+      | inl () => check_if_subkind κ k
+      | err => err
+      end
+  | ExistsMemT κ τ =>
+      match kind_ok_checker (F.(fc_kind_ctx)) κ with
+      | inl () =>
+          match has_kind_checker (F <| fc_kind_ctx ::= set kc_mem_vars S |>) τ κ with
+          | inl () => check_if_subkind κ k
+          | err => err
+          end
+      | err => err
+      end
+  | ExistsRepT κ τ =>
+      match kind_ok_checker (F.(fc_kind_ctx)) κ with
+      | inl () =>
+          match has_kind_checker (F <| fc_kind_ctx ::= set kc_rep_vars S |>) τ κ with
+          | inl () => check_if_subkind κ k
+          | err => err
+          end
+      | err => err
+      end
+   | ExistsSizeT κ τ =>
+      match kind_ok_checker (F.(fc_kind_ctx)) κ with
+      | inl () =>
+          match has_kind_checker (F <| fc_kind_ctx ::= set kc_size_vars S |>) τ κ with
+          | inl () => check_if_subkind κ k
+          | err => err
+          end
+      | err => err
+      end
+  | ExistsTypeT κ κ0 τ =>
+      match kind_ok_checker (F.(fc_kind_ctx)) κ with
+      | inl () =>
+          match kind_ok_checker (F.(fc_kind_ctx)) κ0 with
+          | inl () =>
+              match has_kind_checker (F <| fc_type_vars ::= cons κ0 |>) τ κ with
+              | inl () => check_if_subkind κ k
+              | err => err
+              end
+          | err => err
+          end
+      | err => err
+      end
+  end.
+
+Ltac my_auto3 :=
+  try structural_auto; try boolean_equality_auto; try
+  match goal with
+  | H: (kind_ok_checker _ _ = inl ()) |- _ => apply kind_ok_checker_correct in H; auto
+  | H: (kind_ok_checker _ _ = ok_term) |- _ => apply kind_ok_checker_correct in H; auto
+  | H: (mem_ok_checker _ _ = inl ()) |- _ => apply mem_ok_checker_correct in H; auto
+  | H: (mem_ok_checker _ _ = ok_term) |- _ => apply mem_ok_checker_correct in H; auto
+  | H: (rep_ok_checker _ _ = inl ()) |- _ => apply rep_ok_checker_correct in H; auto
+  | H: (rep_ok_checker _ _ = ok_term) |- _ => apply rep_ok_checker_correct in H; auto
+  | H: (size_ok_checker _ _ = inl ()) |- _ => apply size_ok_checker_correct in H; auto
+  | H: (size_ok_checker _ _ = ok_term) |- _ => apply size_ok_checker_correct in H; auto
+  | H: (type_ok_checker _ _ = inl ()) |- _ => apply type_ok_checker_correct in H; auto
+  | H: (type_ok_checker _ _ = ok_term) |- _ => apply type_ok_checker_correct in H; auto
+  | H: (function_type_ok_checker _ _ = inl ()) |- _ => apply function_type_ok_checker_correct in H; auto
+  | H: (function_type_ok_checker _ _ = ok_term) |- _ => apply function_type_ok_checker_correct in H; auto
+  | H: (check_if_subkind _ _ = inl ()) |- _ =>
+      try( by (eapply check_if_subkind_works_with_has_kind; try constructor; auto))
+  | H: (check_if_subkind _ _ = ok_term) |- _ =>
+      try( by (eapply check_if_subkind_works_with_has_kind; try constructor; auto))
+  | H: (INR _ = ok_term) |- _ => inversion H
+  | H: (INR _ = inl ()) |- _ => inversion H
+end.
+
+Opaque check_if_subkind.
+Opaque mem_ok_checker.
+(* this needs to not be unravelled by any tactics. Makes
+ automation a lot easier *)
+
+
+(* The stupid True is there bc idk how to make the induction work otherwise *)
+Lemma has_kind_checker_correct_basic :
+  (∀ t F k, has_kind_checker F t k = ok_term -> has_kind F t k) /\
+  (∀ (ft:function_type) (F:function_ctx), True  ).
+Proof.
+  apply type_and_function_ind; intros; simpl in *; auto; repeat my_auto3.
+  (* The following 4 (sums and prods) will rely on some foldr2 lemma *)
+  (* I will do that later *)
+  1-4: admit.
+
+  (* then these actually need the simple inductive hyp *)
+  1-3: match goal with
+    | HSTAR: (has_kind_checker _ _ _ = _) |- _ => apply H in HSTAR
+    end.
+
+  1-2: eapply check_if_subkind_works_with_has_kind; [apply H0 | apply (KRef _ _ _ s r); auto].
+  1: eapply check_if_subkind_works_with_has_kind; [apply H0 | apply (KRefGC _ _ s r); auto].
+
+
+Admitted.
+
+Lemma has_kind_checker_correct :
+  ∀ F t k, has_kind_checker F t k = ok_term -> has_kind F t k.
+Proof.
+  pose proof has_kind_checker_correct_basic.
+  destruct H; auto.
+Qed.
+
+
+(* Small things before pathing *)
+Definition has_rep_checker F τ ρ : type_checker_res :=
+  has_kind_checker F τ (VALTYPE ρ NoRefs).
+
+Lemma has_rep_checker_correct :
+  ∀ F τ ρ, has_rep_checker F τ ρ = ok_term -> has_rep F τ ρ.
+Proof.
+  intros.
+  unfold has_rep_checker in H.
+  apply has_kind_checker_correct in H.
+  apply (RepVALTYPE _ _ _ NoRefs); auto.
+Qed.
+
+Definition grab_rep F τ : option representation :=
+  match grab_kind F τ with
+  | Some κ =>
+      match κ with
+      | VALTYPE ρ _  => Some ρ
+      | _ => None
+      end
+  | None => None
+  end.
+
+Definition is_mono_rep_checker :=
+  rep_ok_checker kc_empty.
+
+Definition has_mono_rep_checker F τ : type_checker_res :=
+  match grab_rep F τ with
+  | Some ρ =>
+      match has_rep_checker F τ ρ with
+      | inl () => is_mono_rep_checker ρ
+      | err => err
+      end
+  | None => INR "youre checking mono rep for something that is not valtype or smthn similar"
+  end.
+
+Lemma has_mono_rep_checker_correct :
+  ∀ F τ, has_mono_rep_checker F τ = ok_term -> has_mono_rep F τ.
+Proof.
+  intros. unfold has_mono_rep_checker in H.
+  repeat my_auto3.
+  unfold is_mono_rep_checker in *.
+  repeat my_auto3.
+  apply has_rep_checker_correct in HMatch0.
+  apply (MonoRep _ _ r); auto.
+Qed.
+
+Definition has_mono_rep_instr_checker F inst : type_checker_res :=
+  match inst with
+  | InstrT τs1 τs2 =>
+      if (foldr (λ t:type, andb (check_ok (has_mono_rep_checker F) t)) true τs1)
+      then
+        if (foldr (λ t:type, andb (check_ok (has_mono_rep_checker F) t)) true τs2)
+        then ok_term
+        else INR "function type ok error"
+      else INR "function type ok error"
+  end.
+
+Lemma has_mono_rep_instr_checker_correct :
+  ∀ F inst, has_mono_rep_instr_checker F inst = ok_term -> has_mono_rep_instr F inst.
+Proof.
+  intros.
+  unfold has_mono_rep_instr_checker in *.
+  repeat my_auto3. pose proof has_mono_rep_checker_correct.
+  split; [clear HMatch1 | clear HMatch0].
+  - (* yeah this is true but I dont wanna prove it *)
+    admit.
+  - admit.
+Admitted.
+
+(* I think type_size can do this but oh well *)
+Definition grab_size F τ : option size :=
+  match grab_kind F τ with
+  | Some κ =>
+      match κ with
+      | MEMTYPE σ _ => Some σ
+      | _ => None
+      end
+  | None => None
+  end.
+
+Definition has_size_checker F τ σ : type_checker_res :=
+  has_kind_checker F τ (MEMTYPE σ NoRefs).
+
+Lemma has_size_checker_correct :
+  ∀ F τ σ, has_size_checker F τ σ = ok_term -> has_size F τ σ.
+Proof.
+  intros. unfold has_size_checker in H.
+  apply has_kind_checker_correct in H.
+  unfold has_size.
+  by exists NoRefs.
+Qed.
+
+Definition is_mono_size_checker := size_ok_checker kc_empty.
+
+Definition has_mono_size_checker F τ : type_checker_res :=
+  match grab_size F τ with
+  | Some σ =>
+      match has_size_checker F τ σ with
+      | inl () => is_mono_size_checker σ
+      | err => err
+      end
+  | None => INR "youre checking mono size for something that is not memtype or smthn similar"
+  end.
+
+Lemma has_mono_size_checker_correct :
+  ∀ F τ, has_mono_size_checker F τ = ok_term -> has_mono_size F τ.
+Proof.
+  intros.
+  unfold has_mono_size_checker in *.
+  repeat my_auto3.
+  unfold is_mono_size_checker in *. unfold has_size_checker in *.
+  repeat my_auto3. apply has_kind_checker_correct in HMatch0.
+  by apply (MonoSizeMEMTYPE _ _ s NoRefs).
+Qed.
+
+
+Definition type_rep_eq_prim_checker F τ ηs : type_checker_res :=
+  match grab_rep F τ with
+  | Some ρ =>
+      match has_rep_checker F τ ρ with
+      | inl () =>
+          match eval_rep_prim EmptyEnv ρ with
+          | Some ηs1 =>
+              if list_beq primitive primitive_beq ηs ηs1
+              then ok_term
+              else INR "uh primitives don't match?"
+          | None => INR "bad rep i think"
+          end
+      | err => err
+      end
+  | None => INR "um not valtype?"
+  end.
+
+Lemma type_rep_eq_prim_checker_correct :
+  ∀ F τ ηs, type_rep_eq_prim_checker F τ ηs = ok_term -> type_rep_eq_prim F τ ηs.
+Proof.
+  intros.
+  unfold type_rep_eq_prim_checker in H.
+  repeat my_auto3.
+  apply has_rep_checker_correct in HMatch0. rename l into ηs1.
+  exists r. split; auto.
+  (* give some theorems about list_beq, this is obvious *)
+  admit.
+Admitted.
+
+(* NOTE:  a bit of confusing terminology. size_beq is actual equality.
+ size_eq_checker will be about it evalling to the same n *)
+
+Definition size_eq_checker σ1 σ2 : type_checker_res :=
+  match eval_size EmptyEnv σ1 with
+  | Some n1 =>
+      match eval_size EmptyEnv σ2 with
+      | Some n2 =>
+          if n1 =? n2
+          then ok_term
+          else INR "unequal sizes"
+      | None => INR "bad size"
+      end
+  | None => INR "bad size"
+  end.
+
+Lemma size_eq_checker_correct :
+  ∀ σ1 σ2, size_eq_checker σ1 σ2 = ok_term -> size_eq σ1 σ2.
+Proof.
+  intros. unfold size_eq_checker in *.
+  repeat my_auto3.
+  apply Nat.eqb_eq in HMatch1; subst.
+  econstructor; [apply HMatch | apply HMatch0].
+Qed.
+
+Definition size_leq_checker σ1 σ2 : type_checker_res :=
+  match eval_size EmptyEnv σ1 with
+  | Some n1 =>
+      match eval_size EmptyEnv σ2 with
+      | Some n2 =>
+          if n1 <=? n2
+          then ok_term
+          else INR "unequal sizes"
+      | None => INR "bad size"
+      end
+  | None => INR "bad size"
+  end.
+
+Lemma size_leq_checker_correct :
+  ∀ σ1 σ2, size_leq_checker σ1 σ2 = ok_term -> size_leq σ1 σ2.
+Proof. (* easy *)
+  intros. unfold size_leq_checker in *.
+  repeat my_auto3.
+  apply Nat.leb_le in HMatch1.
+  by (exists n; exists n0).
+Qed.
+
+Definition type_size_eq_checker F τ1 τ2 : type_checker_res :=
+  match grab_size F τ1 with
+  | Some σ1 =>
+      match grab_size F τ2 with
+      | Some σ2 =>
+          match has_size_checker F τ1 σ1 with
+          | inl () =>
+              match has_size_checker F τ2 σ2 with
+              | inl () => size_eq_checker σ1 σ2
+              | err => err
+              end
+          | err => err
+          end
+      | None => INR "bad type for size"
+      end
+  | None => INR "bad type for size"
+  end.
+
+Lemma type_size_eq_checker_correct :
+  ∀ F τ1 τ2, type_size_eq_checker F τ1 τ2 = ok_term -> type_size_eq F τ1 τ2.
+Proof.
+  intros. unfold type_size_eq_checker in H.
+  repeat my_auto3.
+  apply has_size_checker_correct in HMatch1, HMatch2.
+  apply size_eq_checker_correct in H.
+  exists s, s0. split; auto.
+Qed.
+
+(*
+Definition grab_copyability F τ : option copyability :=
+  match grab_kind F τ with
+  | Some (VALTYPE _ χ _) => Some χ
+  | _ => None
+  end.
+
+Definition grab_dropability F τ : option dropability :=
+  match grab_kind F τ with
+  | Some (VALTYPE _ _ δ) => Some δ
+  | Some (MEMTYPE _ δ) => Some δ
+  | None => None
+  end.
+*)
+Definition grab_ref_flag F τ : option ref_flag :=
+  match grab_kind F τ with
+  | Some (VALTYPE _ ξ)
+  | Some (MEMTYPE _ ξ) => Some ξ
+  | None => None
+  end.
+
+(*
+Definition has_copyability_checker F τ χ : type_checker_res :=
+  match grab_rep F τ with
+  | Some ρ => has_kind_checker F τ (VALTYPE ρ χ ImDrop)
+  | None => INR "not valtype"
+  end.
+Lemma has_copyability_checker_correct :
+  ∀ F τ χ, has_copyability_checker F τ χ = ok_term -> has_copyability F τ χ.
+Proof.
+  intros; unfold has_copyability_checker in *.
+  repeat my_auto3.
+  apply has_kind_checker_correct in H.
+  apply (CopyVALTYPE _ _ r _ ImDrop); auto.
+Qed.
+
+Definition has_dropability_checker F τ δ : type_checker_res :=
+  match grab_kind F τ with
+  | Some κ =>
+      match κ with
+      | VALTYPE ρ _ _ => has_kind_checker F τ (VALTYPE ρ ImCopy δ)
+      | MEMTYPE σ _ => has_kind_checker F τ (MEMTYPE σ δ)
+      end
+  | None => INR "bad kind"
+  end.
+
+Lemma has_dropability_checker_correct :
+  ∀ F τ δ, has_dropability_checker F τ δ = ok_term -> has_dropability F τ δ.
+Proof.
+  unfold has_dropability_checker; intros. repeat my_auto3; apply has_kind_checker_correct in H.
+  - by apply (DropVALTYPE _ _ r ImCopy _).
+  - by apply (DropMEMTYPE _ _ s _).
+Qed.
+*)
+Definition has_ref_flag_checker F τ ξ : type_checker_res :=
+  match grab_kind F τ with
+  | Some κ =>
+      match κ with
+      | VALTYPE ρ _ => has_kind_checker F τ (VALTYPE ρ ξ)
+      | MEMTYPE σ _ => has_kind_checker F τ (MEMTYPE σ ξ)
+      end
+  | None => INR "bad kind"
+  end.
+Lemma has_ref_flag_checker_correct :
+  ∀ F τ ξ, has_ref_flag_checker F τ ξ = ok_term -> has_ref_flag F τ ξ.
+Proof.
+  unfold has_ref_flag_checker; intros. repeat my_auto3; apply has_kind_checker_correct in H.
+  - by eapply MemtypeHasRefFlag; auto.
+  - by eapply ValtypeHasRefFlag; auto.
+Qed.
+
+
+(* Resolves path, and some other more complicated stuff before has_instruction_type *)
+
+Fixpoint get_list_of_reps (σs : list size) : option (list representation) :=
+  match σs with
+  | [] => Some []
+  | (RepS ρ) :: σss =>
+      match get_list_of_reps σss with
+      | Some ρs => Some (ρ :: ρs)
+      | None => None
+      end
+  | _ => None
+  end.
+
+Lemma get_list_of_reps_matches_map :
+  (∀ σs ρs, get_list_of_reps σs = Some ρs <-> σs = (map RepS ρs)).
+Proof.
+  split; intros.
+  - generalize dependent ρs.
+    induction σs.
+    + intros. simpl in H. inversion H; subst; simpl; auto.
+    + intros.
+      simpl in H.
+      repeat my_auto3. subst.
+      specialize (IHσs l). specialize (IHσs eq_refl).
+      subst; auto.
+  - generalize dependent ρs.
+    induction σs.
+    + intros. simpl in *.
+      symmetry in H; apply map_eq_nil in H.
+      by subst.
+    + intros; simpl in *.
+      symmetry in H.
+      destruct ρs; [simpl in H; inversion H |].
+      rewrite map_cons in H.
+      inversion H; subst.
+      specialize (IHσs ρs eq_refl).
+      by rewrite IHσs.
+Qed.
+
+
+
+Ltac my_auto3_5 :=
+  try structural_auto; try boolean_equality_auto; try
+  match goal with
+  | H: (kind_ok_checker _ _ = inl ()) |- _ => apply kind_ok_checker_correct in H; auto
+  | H: (kind_ok_checker _ _ = ok_term) |- _ => apply kind_ok_checker_correct in H; auto
+  | H: (mem_ok_checker _ _ = inl ()) |- _ => apply mem_ok_checker_correct in H; auto
+  | H: (mem_ok_checker _ _ = ok_term) |- _ => apply mem_ok_checker_correct in H; auto
+  | H: (rep_ok_checker _ _ = inl ()) |- _ => apply rep_ok_checker_correct in H; auto
+  | H: (rep_ok_checker _ _ = ok_term) |- _ => apply rep_ok_checker_correct in H; auto
+  | H: (size_ok_checker _ _ = inl ()) |- _ => apply size_ok_checker_correct in H; auto
+  | H: (size_ok_checker _ _ = ok_term) |- _ => apply size_ok_checker_correct in H; auto
+  | H: (type_ok_checker _ _ = inl ()) |- _ => apply type_ok_checker_correct in H; auto
+  | H: (type_ok_checker _ _ = ok_term) |- _ => apply type_ok_checker_correct in H; auto
+  | H: (function_type_ok_checker _ _ = inl ()) |- _ => apply function_type_ok_checker_correct in H; auto
+  | H: (function_type_ok_checker _ _ = ok_term) |- _ => apply function_type_ok_checker_correct in H; auto
+  | H: (has_kind_checker _ _ _ = ok_term) |- _ => apply has_kind_checker_correct in H; auto
+  | H: (has_kind_checker _ _ _ = inl ()) |- _ => apply has_kind_checker_correct in H; auto
+  | H: (check_if_subkind _ _ = inl ()) |- _ =>
+      try( by (eapply check_if_subkind_works_with_has_kind; try constructor; auto))
+  | H: (check_if_subkind _ _ = ok_term) |- _ =>
+      try( by (eapply check_if_subkind_works_with_has_kind; try constructor; auto))
+  | H: (INR _ = ok_term) |- _ => inversion H
+  | H: (INR _ = inl ()) |- _ => inversion H
+end.
+
+(* This is an attempt without a double match for the sake of the proof later *)
+Fixpoint type_eq_checker (F:function_ctx) (τ1:type) (τ2:type) :type_checker_res :=
+  (* base cases *)
+  match τ1 with
+  | VarT _ =>
+      match τ2 with
+      | VarT _ => if type_beq τ1 τ2 then ok_term else INR "types not equal"
+      | _ => INR "types note equal"
+      end
+  | I31T _ =>
+      match τ2 with
+      | I31T _ => if type_beq τ1 τ2 then ok_term else INR "types not equal"
+      | _ => INR "types not equal"
+      end
+  | NumT _ _ =>
+      match τ2 with
+      | NumT _ _ => if type_beq τ1 τ2 then ok_term else INR "types not equal"
+      | _ => INR "types note equal"
+      end
+  | CodeRefT _ _ =>
+      match τ2 with
+      | CodeRefT _ _ => if type_beq τ1 τ2 then ok_term else INR "types not equal"
+      | _ => INR "types note equal"
+      end
+  | PlugT _ _ =>
+      match τ2 with
+      | PlugT _ _ => if type_beq τ1 τ2 then ok_term else INR "types not equal"
+      | _ => INR "types note equal"
+      end
+  | SpanT _ _ =>
+      match τ2 with
+      | SpanT _ _ => if type_beq τ1 τ2 then ok_term else INR "types not equal"
+      | _ => INR "types note equal"
+      end
+  (* Recursive cases *)
+  | SumT κ1 τs1 =>
+      match τ2 with
+      | SumT κ2 τs2 =>
+          if kind_beq κ1 κ2
+          then
+            match has_kind_checker F (SumT κ1 τs1) κ1 with
+            | inl () =>
+                if foldr2 (λ τ1, λ τ2, andb (check_ok_output (type_eq_checker F τ1 τ2))) true τs1 τs2
+                then ok_term
+                else INR "types not equal"
+            | err => err
+            end
+          else INR "types not equal"
+      | _ => INR "types not equal"
+      end
+  | VariantT κ1 τs1 =>
+      match τ2 with
+      | VariantT κ2 τs2 =>
+          if kind_beq κ1 κ2
+          then
+            match has_kind_checker F (VariantT κ1 τs1) κ1 with
+            | inl () =>
+                if foldr2 (λ τ1, λ τ2, andb (check_ok_output (type_eq_checker F τ1 τ2))) true τs1 τs2
+                then ok_term
+                else INR "types not equal"
+            | err => err
+            end
+          else INR "types not equal"
+      | _ => INR "types not equal"
+      end
+  | ProdT κ1 τs1 =>
+      match τ2 with
+      | ProdT κ2 τs2 =>
+          if kind_beq κ1 κ2
+          then
+            match has_kind_checker F (ProdT κ1 τs1) κ1 with
+            | inl () =>
+                if foldr2 (λ τ1, λ τ2, andb (check_ok_output (type_eq_checker F τ1 τ2))) true τs1 τs2
+                then ok_term
+                else INR "types not equal"
+            | err => err
+            end
+          else INR "types not equal"
+      | _ => INR "types not equal"
+      end
+  | RefT κ1 μ1 τ1 =>
+      match τ2 with
+      | RefT κ2 μ2 τ2 =>
+          if andb (kind_beq κ1 κ2) (memory_beq μ1 μ2)
+          then
+            match has_kind_checker F (RefT κ1 μ1 τ1) κ1 with
+            | inl () => type_eq_checker F τ1 τ2
+            | err => err
+            end
+          else INR "types not equal"
+      | _ => INR "types not equal"
+      end
+  | RecT κ1 τ1 =>
+      match τ2 with
+      | RecT κ2 τ2 =>
+          if kind_beq κ1 κ2
+          then
+            match has_kind_checker F (RecT κ1 τ1) κ1 with
+            | inl () => type_eq_checker F τ1 τ2
+            | err => err
+            end
+          else INR "types not equal"
+      | _ => INR "types not equal"
+      end
+  | ExistsMemT κ1 τ1 =>
+      match τ2 with
+      | ExistsMemT κ2 τ2 =>
+          if kind_beq κ1 κ2
+          then
+            match has_kind_checker F (ExistsMemT κ1 τ1) κ1 with
+            | inl () => type_eq_checker F τ1 τ2
+            | err => err
+            end
+          else INR "types not equal"
+      | _ => INR "types not equal"
+      end
+  | ExistsRepT κ1 τ1 =>
+      match τ2 with
+      | ExistsRepT κ2 τ2 =>
+          if kind_beq κ1 κ2
+          then
+            match has_kind_checker F (ExistsRepT κ1 τ1) κ1 with
+            | inl () => type_eq_checker F τ1 τ2
+            | err => err
+            end
+          else INR "types not equal"
+      | _ => INR "types not equal"
+      end
+  | ExistsSizeT κ1 τ1 =>
+      match τ2 with
+      | ExistsSizeT κ2 τ2 =>
+          if kind_beq κ1 κ2
+          then
+            match has_kind_checker F (ExistsSizeT κ1 τ1) κ1 with
+            | inl () => type_eq_checker F τ1 τ2
+            | err => err
+            end
+          else INR "types not equal"
+      | _ => INR "types not equal"
+      end
+  | ExistsTypeT κ1 κτ1 τ1 =>
+      match τ2 with
+      | ExistsTypeT κ2 κτ2 τ2 =>
+          if andb (kind_beq κ1 κ2) (kind_beq κτ1 κτ2)
+          then
+            match has_kind_checker F (ExistsTypeT κ1 κτ1 τ1) κ1 with
+            | inl () => type_eq_checker F τ1 τ2
+            | err => err
+            end
+          else INR "types not equal"
+      | _ => INR "types not equal"
+      end
+  | SerT κ1 τ1 =>
+      match τ2 with
+      | SerT κ2 τ2 =>
+          if kind_beq κ1 κ2
+          then
+            match has_kind_checker F (SerT κ1 τ1) κ1 with
+            | inl () => type_eq_checker F τ1 τ2
+            | err => err
+            end
+          else INR "types not equal"
+      | StructT κ2 τs2 =>
+          match τ1 with
+          | ProdT κp τs =>
+              if kind_beq κ1 κ2
+              then (* I now throw away κ' *)
+                match κ1 with
+                | MEMTYPE (ProdS σs) ξ =>
+                    match get_list_of_reps σs with
+                    | Some ρs =>
+                        if foldr2
+                             (λ τ:type, λ ρ:representation,
+                                   andb (check_ok_output (has_kind_checker F τ (VALTYPE ρ ξ)))
+                             ) true τs ρs
+                        then (* now just check that τs' equal to the monstrosity *)
+                          if list_beq type type_beq τs2 ((zip_with (fun τ ρ => SerT (MEMTYPE (RepS ρ) ξ) τ)) τs ρs)
+                          then ok_term
+                          else INR "types not_equal"
+                        else INR "types not equal"
+                    | None => INR "types not equal"
+                    end
+                | _ => INR "types not equal"
+                end
+              else INR "types not equal"
+
+          | _ => INR "types not equal"
+          end
+      | _ => INR "types not equal"
+      end
+  | StructT κ1 τs1 =>
+      match τ2 with
+      | StructT κ2 τs2 =>
+          if kind_beq κ1 κ2
+          then
+            match has_kind_checker F (StructT κ1 τs1) κ1 with
+            | inl () =>
+                if foldr2 (λ τ1, λ τ2, andb (check_ok_output (type_eq_checker F τ1 τ2))) true τs1 τs2
+                then ok_term
+                else INR "types not equal 1"
+            | err => err
+            end
+          else INR "types not equal 2"
+      | SerT κ2 τ2 =>
+          match τ2 with
+          | ProdT κp τs =>
+              if kind_beq κ2 κ1
+              then (* I now throw away κ' *)
+                match κ2 with
+                | MEMTYPE (ProdS σs) ξ =>
+                    match get_list_of_reps σs with
+                    | Some ρs =>
+                        if foldr2
+                             (λ τ:type, λ ρ:representation,
+                                   andb (check_ok_output (has_kind_checker F τ (VALTYPE ρ ξ)))
+                             ) true τs ρs
+                        then (* now just check that τs' equal to the monstrosity *)
+                          if list_beq type type_beq τs1 ((zip_with (fun τ ρ => SerT (MEMTYPE (RepS ρ) ξ) τ)) τs ρs)
+                          then ok_term
+                          else INR "types not_equal 3"
+                        else INR "types not equal 4"
+                    | None => INR "types not equal 5"
+                    end
+                | _ => INR "types not equal 6"
+                end
+              else INR "types not equal 7"
+          | _ => INR "types not equal 8"
+          end
+
+      | _ => INR "types not equal HERE 9"
+      end
+
+  end.
+
+
+
+(* NOTE: the reason this has such a weird set up is because this
+   is the only way I know how to use type_and_function_ind
+
+  also NOTE: this is written more verbosely than ideal due to
+  the automation slowing down a Lot without a bit of help.
+ *)
+Opaque has_kind_checker.
+
+Lemma type_eq_checker_correct_basic :
+  (∀ τ1,
+     (∀ τ2, ∀ F, type_eq_checker F τ1 τ2 = ok_term -> type_eq F τ1 τ2)
+  ) /\
+  (∀ ft:function_type, True).
+Proof.
+  apply type_and_function_ind; auto; intros; destruct τ2.
+  (* the goal of this big guy: filter all obvious ones. Does not include "obvious" Ser *)
+  all:
+    match goal with
+    | |- (type_eq _ (VarT _) (VarT _)) => simpl in H; repeat my_auto3_5; apply TEqRefl
+    | |- (type_eq _ (I31T _) (I31T _)) => simpl in H; repeat my_auto3_5; apply TEqRefl; auto
+    | |- (type_eq _ (NumT _ _) (NumT _ _)) => simpl in H; repeat my_auto3_5; apply TEqRefl; repeat my_auto3_5
+    | |- (type_eq _ (SumT _ _) (SumT _ _)) => idtac
+    | |- (type_eq _ (VariantT _ _) (VariantT _ _)) => idtac
+    | |- (type_eq _ (ProdT _ _) (ProdT _ _)) => idtac
+    | |- (type_eq _ (StructT _ _) (StructT _ _)) => idtac
+    | |- (type_eq _ (RefT _ _ _) (RefT _ _ _)) =>
+        simpl in H0; repeat my_auto3_5; apply H in H0; apply TEqRef; auto
+    | |- (type_eq _ (CodeRefT _ _) (CodeRefT _ _)) => simpl in *; repeat my_auto3_5; apply TEqRefl; auto
+    | |- (type_eq _ (SerT _ _) (SerT _ _)) =>
+        simpl in H0; repeat my_auto3_5; apply TEqSer; auto
+    | |- (type_eq _ (StructT _ _) (SerT _ _)) => idtac
+    | |- (type_eq _ (SerT _ _) (StructT _ _)) => idtac
+    | |- (type_eq _ (SerT _ _) _) => simpl in H0; my_auto3_5
+    | |- (type_eq _ (PlugT _ _) (PlugT _ _)) => simpl in *; repeat my_auto3_5; apply TEqRefl; auto
+    | |- (type_eq _ (SpanT _ _) (SpanT _ _)) => simpl in *; repeat my_auto3_5; apply TEqRefl; auto
+    | |- (type_eq _ (RecT _ _) (RecT _ _)) =>
+        simpl in H0; repeat my_auto3_5; apply H in H0; apply TEqRec; auto
+    | |- (type_eq _ (ExistsMemT _ _) (ExistsMemT _ _)) =>
+        simpl in H0; repeat my_auto3_5; apply H in H0; apply TEqExMem; auto
+    | |- (type_eq _ (ExistsRepT _ _) (ExistsRepT _ _)) =>
+        simpl in H0; repeat my_auto3_5; apply H in H0; apply TEqExRep; auto
+    | |- (type_eq _ (ExistsSizeT _ _) (ExistsSizeT _ _)) =>
+        simpl in H0; repeat my_auto3_5; apply H in H0; apply TEqExSize; auto
+    | |- (type_eq _ (ExistsTypeT _ _ _) (ExistsTypeT _ _ _)) =>
+        simpl in H0; repeat my_auto3_5; apply H in H0; apply TEqExType; auto
+    | _ => simpl in *; my_auto3_5
+    end.
+
+  all: idtac. (* this is here because doom emacs despises the match goal above *)
+
+  (* struct ser case *)
+  6: {
+    simpl in H0. destruct τ2; simpl in H0; repeat my_auto3_5.
+    apply get_list_of_reps_matches_map in HMatch1; subst.
+    apply TEqSym.
+    apply (TEqSerProd _ _ l1 r _).
+    (* this then relies on some foldr2 lemmas *)
+    admit.
+  }
+  (* ser struct case *)
+  6: {
+    Opaque has_kind_checker.
+    simpl in H0. destruct t; simpl in H0; repeat my_auto3_5.
+    apply get_list_of_reps_matches_map in HMatch1; subst.
+    apply (TEqSerProd _ _ l2 r _).
+    (* this then relies on some foldr2 lemmas *)
+    admit.
+
+  }
+  (* All the rest of are foldr2 lemma reliant, so *)
+  all: admit.
+
+Admitted.
+
+
+Lemma type_eq_checker_correct :
+  ∀ F τ1 τ2, type_eq_checker F τ1 τ2 = ok_term -> type_eq F τ1 τ2.
+Proof.
+  pose proof type_eq_checker_correct_basic.
+  destruct H as [H1 H2].
+  intros.
+  specialize (H1 τ1).
+  auto.
+Qed.
+
+Fixpoint split_into_three (τs:list type) (i:nat) : option (list type * type * list type) :=
+  match i with
+  | O =>
+      match τs with
+      | [] => None
+      | τ :: τs' => Some ([], τ, τs')
+      end
+  | S n =>
+      match τs with
+      | [] => None
+      | t :: ts =>
+          match split_into_three ts n with
+          | None => None
+          | Some (τs0, τ, τs) => Some (t :: τs0, τ, τs)
+          end
+      end
+  end.
+
+Lemma split_into_three_correct :
+  ∀ τs i τs0 τ τs',
+    split_into_three τs i = Some (τs0, τ, τs') ->
+    Init.Datatypes.length τs0 = i /\ τs = τs0 ++ τ :: τs'.
+Proof.
+  intros τs. induction τs.
+  - intros. destruct i; simpl in H; try inversion H.
+  - intros. destruct i; simpl in H.
+    + inversion H; subst.
+      split; auto.
+    + structural_auto. clear H1.
+      destruct p. destruct p.
+      apply IHτs in HMatch. destruct HMatch as [HL Hyeah].
+      inversion H.
+      subst.
+      split; auto.
+Qed.
+
+Fixpoint list_prefix (lfull lpre : list type) : option (list type) :=
+  match lfull, lpre with
+  | τ1 :: fullrest, τ2 :: prerest =>
+      if type_beq τ1 τ2
+      then list_prefix fullrest prerest
+      else None
+  | lfull, [] => Some lfull
+  | _, _ => None
+  end.
+
+Lemma list_prefix_correct_for :
+  ∀ lfull lpre lsuff,
+    list_prefix lfull lpre = Some lsuff -> lfull = lpre ++ lsuff.
+Proof.
+  induction lfull.
+  - intros. destruct lpre, lsuff; simpl in H; try inversion H. auto.
+  - intros.
+    destruct lpre.
+    + simpl in *. inversion H; auto.
+    + simpl in *. structural_auto. clear H1.
+      apply IHlfull in H. boolean_equality_auto.
+Qed.
+
+Lemma list_prefix_correct_back :
+  ∀ lfull lpre lsuff,
+    lfull = lpre ++ lsuff -> list_prefix lfull lpre = Some lsuff.
+Proof.
+  induction lfull.
+  - intros. destruct lpre, lsuff; try inversion H. auto.
+  - intros.
+    destruct lpre.
+    + simpl. rewrite app_nil_l in H. subst; auto.
+    + inversion H; subst.
+      specialize (IHlfull lpre lsuff eq_refl).
+      simpl.
+      assert (Stupid:t=t) by auto; apply type_eq_convert in Stupid.
+      rewrite Stupid. auto.
+Qed.
+
+Fixpoint resolves_path_checker
+  (τ:type) (p:path) (oτ:option type) (pr':path_result) : type_checker_res :=
+  match p with
+  | [] =>
+      match oτ with
+      | Some τ' =>
+          if path_result_beq pr' (Build_path_result [] τ τ')
+          then ok_term
+          else INR "does not resolve path"
+      | None =>
+          if path_result_beq pr' (Build_path_result [] τ τ)
+          then ok_term
+          else INR "does not resolve path"
+      end
+  | i :: p =>
+      match τ with
+      | StructT κ τs_full =>
+          match split_into_three τs_full i with
+          | Some (τs0, τ_inner, τs') =>
+              match list_prefix pr'.(pr_prefix) τs0 with
+              | Some prprefix =>
+                  match pr'.(pr_replaced) with
+                  | StructT κ0 inner_τs =>
+                      if kind_beq κ κ0
+                      then
+                      match split_into_three inner_τs i with
+                      | Some (τs0', prreplaced, τs'') =>
+                          if andb (list_beq type type_beq τs0 τs0') (list_beq type type_beq τs' τs'')
+                          then
+                            let pr := {| pr_prefix := prprefix;
+                                         pr_target := pr'.(pr_target);
+                                         pr_replaced := prreplaced |} in
+                            resolves_path_checker τ_inner p oτ pr
+                          else INR "bad path resolution"
+                      | None => INR "bad replacement or smthn"
+                      end
+                      else INR "bad path stuff"
+                  | _ => INR "improper path replacement"
+                  end
+              | None => INR "can't prefix?"
+              end
+          | None => INR "does not resolve path"
+          end
+      | _ => INR "does not resolves path"
+      end
+  end.
+Lemma resolves_path_checker_correct_basic :
+  ∀ p τ oτ pres, resolves_path_checker τ p oτ pres = ok_term -> resolves_path τ p oτ pres.
+Proof.
+  intros p.
+  induction p.
+  - intros. unfold resolves_path_checker in H.
+    destruct oτ; repeat my_auto3_5.
+    + apply PathNilSome.
+    + apply PathNilNone.
+  - intros.
+    simpl in H. Opaque resolves_path_checker.
+    repeat structural_auto. subst.
+    clear H1 H2 H3 H4 H5 H6 H7 H8 H9 H10.
+    repeat boolean_equality_auto; subst.
+    rename l into τs_full; rename a into i; rename l5 into τs0; rename l4 into τs'.
+    rename l2 into prprefix. apply list_prefix_correct_for in HMatch3. rename l3 into oldprreplaced.
+    apply split_into_three_correct in HMatch0, HMatch6. destruct HMatch0 as [Hlen Htsfull].
+    destruct HMatch6 as [_ Holdpr]. rename k0 into k.
+    set (pr := {| pr_prefix := prprefix; pr_target := pr_target pres; pr_replaced := t0 |}).
+    assert (Hmaybe : pres =
+                       {| pr_prefix := τs0 ++ pr.(pr_prefix);
+                          pr_target := pr.(pr_target);
+                          pr_replaced := StructT k (τs0 ++ pr.(pr_replaced) :: τs')
+                       |}
+           ).
+    {
+      destruct pres. subst.
+      simpl in *. subst. auto.
+    }
+    rewrite Htsfull. rewrite Hmaybe.
+    apply (PathStruct pr i p oτ τs0 t τs' k); auto.
+
+Qed.
+
+Lemma resolves_path_checker_correct :
+  ∀ τ p oτ pres, resolves_path_checker τ p oτ pres = ok_term -> resolves_path τ p oτ pres.
+Proof. intros. apply resolves_path_checker_correct_basic. auto. Qed.
+
+Fixpoint synth_resolving_path
+  (τ:type) (p:path) (oτ:option type) : option path_result :=
+  match p with
+  | [] =>
+      match oτ with
+      | Some τ' => Some (Build_path_result [] τ τ')
+      | None => Some (Build_path_result [] τ τ)
+      end
+  | i :: p =>
+      match τ with
+      | StructT κ τs_full =>
+          match split_into_three τs_full i with
+          | Some (τs0, τ_inner, τs') =>
+              match synth_resolving_path τ_inner p oτ with
+              | Some pr =>
+                  let pr' :=
+                    {| pr_prefix := τs0 ++ pr.(pr_prefix);
+                      pr_target := pr.(pr_target);
+                      pr_replaced := StructT κ (τs0 ++ pr.(pr_replaced) :: τs') |} in
+                  Some pr'
+              | None => None
+              end
+          | None => None
+          end
+      | _ => None
+      end
+  end
+.
+Lemma synth_resolving_path_correct :
+  ∀ p τ oτ pres, synth_resolving_path τ p oτ = Some pres -> resolves_path τ p oτ pres.
+Proof.
+  induction p.
+  - intros. destruct oτ.
+    + simpl in H. inversion H; subst. constructor.
+    + simpl in H; inversion H; subst. constructor.
+  - intros. simpl in H. repeat structural_auto. clear H H1 H2 H3 H4.
+    apply IHp in HMatch3.
+    apply split_into_three_correct in HMatch0. destruct HMatch0 as [Hlen Hsubs].
+    subst.
+    constructor; auto.
+Qed.
+
+(* This is hyper specific fixpoint, used for TStoreStrong *)
+Fixpoint synth_resolving_with_outer_replaced
+  (τ:type) (p:path) (prreplaced:type) (τval:type) : option (path_result * kind) :=
+  match p with
+  | [] =>
+      match prreplaced with
+      | SerT κser τval_inner =>
+          if type_beq τval τval_inner
+          then Some (Build_path_result [] τ (SerT κser τval), κser)
+          else None
+      | _ => None
+      end
+  | i :: p =>
+      match τ with
+      | StructT κ τs_full =>
+          match split_into_three τs_full i with
+          | Some (τs0, τ_inner, τs') =>
+              match prreplaced with
+              | StructT κ' τs_full' =>
+                  match split_into_three τs_full' i with
+                  | Some (τs0', innerprreplaced, τs'') =>
+                      if andb (andb (list_beq type type_beq τs0 τs0') (kind_beq κ κ'))
+                              (list_beq type type_beq τs' τs'')
+                      then
+                        match synth_resolving_with_outer_replaced τ_inner p innerprreplaced τval with
+                        | Some (pr, κser) =>
+                            let pr' :=
+                              {| pr_prefix := τs0 ++ pr.(pr_prefix);
+                                pr_target := pr.(pr_target);
+                                pr_replaced := StructT κ (τs0 ++ pr.(pr_replaced) :: τs') |} in
+                            Some (pr', κser)
+                        | None => None
+                        end
+                      else None
+                  | None => None
+                  end
+              | _ => None
+              end
+          | None => None
+          end
+      | _ => None
+      end
+
+  end.
+
+Lemma synth_resolving_with_outer_replaced_correct :
+  ∀ p τ prreplaced τval pr κser,
+    synth_resolving_with_outer_replaced τ p prreplaced τval = Some (pr, κser) ->
+    resolves_path τ p (Some (SerT κser τval)) pr /\ pr.(pr_replaced) = prreplaced.
+Proof.
+  induction p.
+  - intros. destruct prreplaced; simpl in *; try inversion H. repeat structural_auto. split.
+    + constructor.
+    + boolean_equality_auto.
+  - intros. simpl in H. repeat structural_auto.
+    apply split_into_three_correct in HMatch0; destruct HMatch0 as [Hlen Htosubst].
+    apply split_into_three_correct in HMatch4; destruct HMatch4 as [Hlen' Htosubst'].
+    repeat boolean_equality_auto.
+    apply IHp in HMatch7 as [ha hi].
+    split.
+    + constructor; auto.
+    + subst; auto.
+Qed.
+
+Definition grab_inner_ft (ft:function_type) : option function_type :=
+  match ft with
+  | ForallMemT ϕ
+  | ForallRepT ϕ
+  | ForallSizeT ϕ
+  | ForallTypeT _ ϕ => Some ϕ
+  | MonoFunT _ _ => None
+  end.
+
+Ltac my_auto4 :=
+  try structural_auto; try boolean_equality_auto; try
+  match goal with
+  | H: (kind_ok_checker _ _ = inl ()) |- _ => apply kind_ok_checker_correct in H; auto
+  | H: (kind_ok_checker _ _ = ok_term) |- _ => apply kind_ok_checker_correct in H; auto
+  | H: (mem_ok_checker _ _ = inl ()) |- _ => apply mem_ok_checker_correct in H; auto
+  | H: (mem_ok_checker _ _ = ok_term) |- _ => apply mem_ok_checker_correct in H; auto
+  | H: (rep_ok_checker _ _ = inl ()) |- _ => apply rep_ok_checker_correct in H; auto
+  | H: (rep_ok_checker _ _ = ok_term) |- _ => apply rep_ok_checker_correct in H; auto
+  | H: (size_ok_checker _ _ = inl ()) |- _ => apply size_ok_checker_correct in H; auto
+  | H: (size_ok_checker _ _ = ok_term) |- _ => apply size_ok_checker_correct in H; auto
+  | H: (type_ok_checker _ _ = inl ()) |- _ => apply type_ok_checker_correct in H; auto
+  | H: (type_ok_checker _ _ = ok_term) |- _ => apply type_ok_checker_correct in H; auto
+  | H: (function_type_ok_checker _ _ = inl ()) |- _ => apply function_type_ok_checker_correct in H; auto
+  | H: (function_type_ok_checker _ _ = ok_term) |- _ => apply function_type_ok_checker_correct in H; auto
+  | H: (has_kind_checker _ _ _ = inl ()) |- _ => apply has_kind_checker_correct in H; auto
+  | H: (has_kind_checker _ _ _ = ok_term) |- _ => apply has_kind_checker_correct in H; auto
+  | H: (check_if_subkind _ _ = inl ()) |- _ =>
+      try( by (eapply check_if_subkind_works_with_has_kind; try constructor; auto))
+  | H: (check_if_subkind _ _ = ok_term) |- _ =>
+      try( by (eapply check_if_subkind_works_with_has_kind; try constructor; auto))
+end.
+
+Definition function_type_inst_checker
+  (F:function_ctx) (i:index) (ft1:function_type) (ft2:function_type) : type_checker_res :=
+  match i with
+  | MemI μ =>
+      match ft1 with
+      | ForallMemT ϕ =>
+          if function_type_beq ft2 (subst_function_type (unscoped.scons μ VarM) VarR VarS VarT ϕ)
+          then ok_term
+          else INR "something not matching in function type inst checker"
+      | _ => INR "bad function type inst"
+      end
+  | RepI ρ =>
+      match ft1 with
+      | ForallRepT ϕ =>
+          if function_type_beq ft2 (subst_function_type VarM (unscoped.scons ρ VarR) VarS VarT ϕ)
+          then ok_term
+          else INR "something not matching in function type inst checker"
+      | _ => INR "bad function type inst"
+      end
+  | SizeI σ =>
+      match ft1 with
+      | ForallSizeT ϕ =>
+          if function_type_beq ft2 (subst_function_type VarM VarR (unscoped.scons σ VarS) VarT ϕ)
+          then ok_term
+          else INR "something not matching in function type inst checker"
+      | _ => INR "bad function type inst"
+      end
+ | TypeI τ =>
+       match ft1 with
+      | ForallTypeT κ ϕ =>
+          match has_kind_checker F τ κ with
+          | inl () =>
+              if function_type_beq ft2 (subst_function_type VarM VarR VarS (unscoped.scons τ VarT) ϕ)
+              then ok_term
+              else INR "something not matching in function type inst checker"
+          | err => err
+          end
+      | _ => INR "bad function type inst"
+      end
+ end.
+
+
+Lemma function_type_inst_checker_correct :
+  ∀ F i ft1 ft2, function_type_inst_checker F i ft1 ft2 = ok_term -> function_type_inst F i ft1 ft2.
+Proof.
+  unfold function_type_inst_checker; intros.
+  repeat my_auto4.
+  all: constructor; auto.
+Qed.
+
+Definition grab_substed_ft F (ix:index) (ft1:function_type) : option function_type :=
+  match ix with
+  | MemI μ =>
+      match ft1 with
+      | ForallMemT ϕ => Some (subst_function_type (unscoped.scons μ VarM) VarR VarS VarT ϕ)
+      | _ => None
+      end
+  | RepI ρ =>
+      match ft1 with
+      | ForallRepT ϕ => Some (subst_function_type VarM (unscoped.scons ρ VarR) VarS VarT ϕ)
+      | _ => None
+      end
+  | SizeI σ =>
+      match ft1 with
+      | ForallSizeT ϕ => Some (subst_function_type VarM VarR (unscoped.scons σ VarS) VarT ϕ)
+      | _ => None
+      end
+ | TypeI τ =>
+       match ft1 with
+      | ForallTypeT κ ϕ =>
+          match has_kind_checker F τ κ with
+          | inl () => Some (subst_function_type VarM VarR VarS (unscoped.scons τ VarT) ϕ)
+          | _ => None
+          end
+      | _ => None
+      end
+  end.
+
+Fixpoint function_type_insts_checker
+      (F:function_ctx) (iss:list index) (ft1:function_type) (ft2:function_type) : type_checker_res :=
+  match iss with
+  | [] =>
+      if function_type_beq ft1 ft2
+      then ok_term
+      else INR "not equal in function_type_insts_checker"
+  | ix :: ixs =>
+      match grab_substed_ft F ix ft1 with
+      | Some ftinner =>
+          match function_type_inst_checker F ix ft1 ftinner with
+          | inl () => function_type_insts_checker F ixs ftinner ft2
+          | err => err
+          end
+      | None => INR "can't find ϕ' for FTCons"
+      end
+  end.
+
+Lemma function_type_insts_checker_correct :
+  ∀ F iss ft1 ft2, function_type_insts_checker F iss ft1 ft2 = ok_term ->
+                   function_type_insts F iss ft1 ft2.
+Proof.
+  intros F iss.
+  induction iss; intros; unfold function_type_insts_checker in H; repeat my_auto4.
+  - constructor.
+  - apply function_type_inst_checker_correct in HMatch0.
+    apply (FTCons _ _ f _ _ _); auto.
+Qed.
+
+
+(* TODO THIS IS SOMETHING I ACTUALLY AM UNSURE HOW TO DO *)
+Definition packed_existential_checker (F:function_ctx) (τ1 τ2:type) : type_checker_res :=
+  match τ2 with
+  | ExistsMemT κ' τ' =>
+      match has_kind_checker F τ' κ' with
+      | inl () =>
+          if true (* TODO HOW DO I GET THE MU OUT OF THERE *)
+            (*list_beq τ1 (subst_type (unscoped.scons μ VarM) VarR VarS VarT τ')*)
+          then ok_term
+          else INR "bad packed existential"
+      | err => err
+      end
+  | ExistsRepT κ' τ' => INR "incomplete"
+  | ExistsSizeT κ' τ' => INR "incomplete"
+  | ExistsTypeT κ' κ τ' => INR "incomplete"
+  | _ => INR "trying to check existential type, but not existential"
+  end.
+
+Lemma packed_existential_checker_correct :
+  ∀ F τ1 τ2, packed_existential_checker F τ1 τ2 = ok_term -> packed_existential F τ1 τ2.
+Proof.
+
+Admitted.
+
+
+(* This one has the reverse list stuff which I'm unsure how to do exactly *)
+Definition unpacked_existential_checker
+ (F:function_ctx) (L1:local_ctx) (insts:list instruction) (instt : instruction_type) (L2:local_ctx)
+ (F':function_ctx) (L1':local_ctx) (insts':list instruction) (instt': instruction_type) (L2':local_ctx)
+  :=
+  INR "incomplete".
+
+Lemma unpacked_existential_checker_correct :
+  ∀ F L1 insts instt L2 F' L1' insts' instt' L2',
+    unpacked_existential_checker F L1 insts instt L2 F' L1' insts' instt' L2' = ok_term ->
+    unpacked_existential F L2 insts instt L2 F' L1' insts' instt' L2'.
+Proof. Admitted.
+
+Definition local_ctx_ok_checker (F:function_ctx) (L:local_ctx) : type_checker_res :=
+  if foldr2
+       (λ t:type, λ p:list primitive,
+             andb (check_ok_output (type_rep_eq_prim_checker F t p))
+       ) true L (F.(fc_locals))
+  then ok_term
+  else INR "local context not ok".
+Lemma local_ctx_ok_checker_correct :
+  ∀ F L, local_ctx_ok_checker F L = ok_term -> local_ctx_ok F L.
+Proof.
+  (* this will be some foldr2 lemmas *)
+Admitted.
+
+
+
+
+
+(* And from here on, we move onto has_instruction_type stuff *)
+Definition has_instruction_type_ok_checker F ψ L' : type_checker_res :=
+  match has_mono_rep_instr_checker F ψ with
+  | inl () => local_ctx_ok_checker F L'
+  | err => err
+  end.
+Lemma has_instruction_type_ok_checker_correct :
+  ∀ F ψ L', has_instruction_type_ok_checker F ψ L' = ok_term -> has_instruction_type_ok F ψ L'.
+Proof.
+  intros. unfold has_instruction_type_ok_checker in H.
+  repeat my_auto3.
+  apply has_mono_rep_instr_checker_correct in HMatch.
+  apply local_ctx_ok_checker_correct in H.
+  constructor; auto.
+Qed.
+
+
+(* NOTE: the reason I do InstrT [a] [b] for most of these is to speed up
+   the automation in the proof. Using the if then else is faster than
+   a match.
+   It also allows me to use the type functions/variables, (like type_i32)
+   rather than fully spelling out the type.
+ *)
+Definition has_instruction_type_cvt_checker cop ψ : type_checker_res :=
+  match cop with
+  | CWrap =>
+      match ψ with
+      | InstrT [a] [b] =>
+          if andb (type_beq a type_i64) (type_beq b type_i32)
+          then ok_term
+          else INR "incorrect cvt instruction type"
+      | _ => INR "incorrect cvt instruction type"
+      end
+  | CExtend _ =>
+      match ψ with
+      | InstrT [a] [b] =>
+          if andb (type_beq a type_i32) (type_beq b type_i64)
+          then ok_term
+          else INR "incorrect cvt instruction type"
+      | _ => INR "incorrect cvt instruction type"
+      end
+  | CTrunc vf vi _ =>
+      match ψ with
+      | InstrT [a] [b] =>
+          if andb (type_beq a (float_type_type vf)) (type_beq b (int_type_type vi))
+          then ok_term
+          else INR "incorrect cvt instruction type"
+      | _ => INR "incorrect cvt instruction type"
+      end
+  | CDemote =>
+      match ψ with
+      | InstrT [a] [b] =>
+          if andb (type_beq a type_f64) (type_beq b type_f32)
+          then ok_term
+          else INR "incorrect cvt instruction type"
+      | _ => INR "incorrect cvt instruction type"
+      end
+  | CPromote =>
+      match ψ with
+      | InstrT [a] [b] =>
+          if andb (type_beq a type_f32) (type_beq b type_f64)
+          then ok_term
+          else INR "incorrect cvt instruction type"
+      | _ => INR "incorrect cvt instruction type"
+      end
+  | CConvert vf vi _ =>
+      match ψ with
+      | InstrT [a] [b] =>
+          if andb (type_beq a (int_type_type vf)) (type_beq b (float_type_type vi))
+          then ok_term
+          else INR "incorrect cvt instruction type"
+      | _ => INR "incorrect cvt instruction type"
+      end
+  | CReinterpret (IntT I32T) =>
+      match ψ with
+      | InstrT [a] [b] =>
+          if andb (type_beq a type_i32) (type_beq b type_f32)
+          then ok_term
+          else INR "incorrect cvt instruction type"
+      | _ => INR "incorrect cvt instruction type"
+      end
+  | CReinterpret (IntT I64T) =>
+      match ψ with
+      | InstrT [a] [b] =>
+          if andb (type_beq a type_i64) (type_beq b type_f64)
+          then ok_term
+          else INR "incorrect cvt instruction type"
+      | _ => INR "incorrect cvt instruction type"
+      end
+  | CReinterpret (FloatT F32T) =>
+      match ψ with
+      | InstrT [a] [b] =>
+          if andb (type_beq a type_f32) (type_beq b type_i32)
+          then ok_term
+          else INR "incorrect cvt instruction type"
+      | _ => INR "incorrect cvt instruction type"
+      end
+  | CReinterpret (FloatT F64T) =>
+      match ψ with
+      | InstrT [a] [b] =>
+          if andb (type_beq a type_f64) (type_beq b type_i64)
+          then ok_term
+          else INR "incorrect cvt instruction type"
+      | _ => INR "incorrect cvt instruction type"
+      end
+  end.
+Lemma has_instruction_type_cvt_checker_correct :
+  ∀ cop ψ, has_instruction_type_cvt_checker cop ψ = ok_term -> has_instruction_type_cvt cop ψ.
+Proof.
+  intros. destruct cop; simpl in *; repeat my_auto4; subst; constructor.
+Qed.
+
+Definition has_instruction_type_num_checker ni ψ :=
+  match ni with
+  | IInt1 vi _ =>
+      match ψ with
+      | InstrT [a] [b] =>
+          if andb (type_beq a (int_type_type vi)) (type_beq b (int_type_type vi))
+          then ok_term
+          else INR "incorrect num instruction type[<35;19;60M]"
+      | _ => INR "incorrect num instruction type"
+      end
+  | IInt2 vi _ =>
+      match ψ with
+      | InstrT [a1; a2] [b] =>
+          if andb (andb (type_beq a1 (int_type_type vi)) (type_beq a2 (int_type_type vi)))
+                  (type_beq b (int_type_type vi))
+          then ok_term
+          else INR "incorrect num instruction type[<35;19;60M]"
+      | _ => INR "incorrect num instruction type"
+      end
+  | IIntTest vi _ =>
+      match ψ with
+      | InstrT [a] [b] =>
+          if andb (type_beq a (int_type_type vi)) (type_beq b type_i32)
+          then ok_term
+          else INR "incorrect num instruction type[<35;19;60M]"
+      | _ => INR "incorrect num instruction type"
+      end
+  | IIntRel vi _ =>
+      match ψ with
+      | InstrT [a1; a2] [b] =>
+          if andb (andb (type_beq a1 (int_type_type vi)) (type_beq a2 (int_type_type vi)))
+                  (type_beq b type_i32)
+          then ok_term
+          else INR "incorrect num instruction type[<35;19;60M]"
+      | _ => INR "incorrect num instruction type"
+      end
+  | IFloat1 vi _ =>
+      match ψ with
+      | InstrT [a] [b] =>
+          if andb (type_beq a (float_type_type vi)) (type_beq b (float_type_type vi))
+          then ok_term
+          else INR "incorrect num instruction type[<35;19;60M]"
+      | _ => INR "incorrect num instruction type"
+      end
+  | IFloat2 vi _ =>
+      match ψ with
+      | InstrT [a1; a2] [b] =>
+          if andb (andb (type_beq a1 (float_type_type vi)) (type_beq a2 (float_type_type vi)))
+                  (type_beq b (float_type_type vi))
+          then ok_term
+          else INR "incorrect num instruction type[<35;19;60M]"
+      | _ => INR "incorrect num instruction type"
+      end
+  | IFloatRel vi _ =>
+      match ψ with
+      | InstrT [a1; a2] [b] =>
+          if andb (andb (type_beq a1 (float_type_type vi)) (type_beq a2 (float_type_type vi)))
+                  (type_beq b type_i32)
+          then ok_term
+          else INR "incorrect num instruction type[<35;19;60M]"
+      | _ => INR "incorrect num instruction type"
+      end
+  | ICvt op => has_instruction_type_cvt_checker op ψ
+  end.
+Lemma has_instruction_type_num_checker_correct :
+  ∀ ni ψ, has_instruction_type_num_checker ni ψ = ok_term -> has_instruction_type_num ni ψ.
+Proof.
+  intros. destruct ni; simpl in *; repeat my_auto4; subst; try constructor.
+  apply has_instruction_type_cvt_checker_correct in H; auto.
+Qed.
+
+(* You know all the previous should have instead been using an instruction_type_beq. Oops.*)
+
+
+(* I'm going to do this really stupidly *)
+Definition has_num_type_type (τ:type) : bool :=
+  orb (orb (type_beq τ (NumT (VALTYPE (AtomR I32R) NoRefs) (IntT I32T)))
+           (type_beq τ (NumT (VALTYPE (AtomR I64R) NoRefs) (IntT I64T))))
+      (orb (type_beq τ (NumT (VALTYPE (AtomR F32R) NoRefs) (FloatT F32T)))
+           (type_beq τ (NumT (VALTYPE (AtomR F64R) NoRefs) (FloatT F64T)))).
+Lemma has_num_type_type_correct :
+  ∀ τ, has_num_type_type τ = true <-> (∃ ν, τ = num_type_type ν).
+Proof.
+  split; intros; unfold has_num_type_type in *.
+  - apply orb_true_iff in H; destruct H as [H | H]; apply orb_true_iff in H; destruct H as [H | H];
+    apply type_eq_convert in H; subst.
+    + exists (IntT I32T); auto.
+    + exists (IntT I64T); auto.
+    + exists (FloatT F32T); auto.
+    + exists (FloatT F64T); auto.
+  - repeat rewrite orb_true_iff.
+    destruct H as [ν H].
+    destruct ν; [destruct i | destruct f].
+    + left; left. by apply type_eq_convert.
+    + left; right. by apply type_eq_convert.
+    + right; left. by apply type_eq_convert.
+    + right; right. by apply type_eq_convert.
+Qed.
+
+
+
+Fixpoint split_list_all_last {A:Type} (l:list A) : option (list A * A) :=
+  match l with
+  | [] => None
+  | [a] => Some ([], a)
+  | h :: rest =>
+      match split_list_all_last rest with
+      | Some (ll, last) => Some (h::ll, last)
+      | None => None
+      end
+  end.
+
+Lemma split_list_all_last_correct :
+  ∀ (A:Type) (l ls:list A) (last:A),
+    split_list_all_last l = Some (ls, last) -> l = ls ++ [last].
+Proof.
+  intros A l.
+  induction l.
+  - intros. simpl in H; inversion H.
+  - intros.
+    simpl in H.
+    destruct l.
+    + inversion H; subst.
+      by rewrite app_nil_l.
+    + my_auto4.
+      clear H1.
+      destruct p. inversion H. subst.
+      specialize (IHl l0 last0 eq_refl).
+      rewrite IHl. auto.
+Qed.
+
+Fixpoint list_suffix_helper (l1 l2: list type) (l1len l2len: nat) : option (list type) :=
+  if l1len =? l2len
+  then
+    if list_beq type type_beq l1 l2
+    then Some []
+    else None
+  else
+    match l1, l1len with
+    | h::rest, S n =>
+        match list_suffix_helper rest l2 n l2len with
+        | Some pr => Some (h::pr)
+        | None => None
+        end
+    | _, _ => None
+    end.
+
+Definition list_suffix l1 l2 : option (list type) :=
+  let l1len := Init.Datatypes.length l1 in
+  let l2len := Init.Datatypes.length l2 in
+  list_suffix_helper l1 l2 l1len l2len.
+
+Lemma list_suffix_correct :
+  ∀ lfull lpre lsuf,
+    lfull = lpre ++ lsuf -> list_suffix lfull lsuf = Some lpre.
+Proof.
+  intros lfull.
+  induction lfull.
+  - intros.
+    destruct lpre, lsuf; try inversion H.
+    auto.
+  - intros lprebig.
+    destruct lprebig as [ | a' lpre ].
+    + admit.
+    + intros.
+      inversion H; subst.
+      specialize (IHlfull lpre lsuf eq_refl).
+      (* yeah this is right, I just need theorems about lengths of lists *)
+      admit.
+Admitted.
+
+(*Definition get_instruction_type_arity (ψ:instruction_type) : nat * nat :=
+  match ψ with
+  | InstrT τs1 τs2 => (Init.Datatypes.length τs1, Init.Datatypes.length τs2)
+  end.*)
+
+(* inl means no error. None just means can't synth (uncreachable,
+   break, return). inr means error in synthesizing (possible in
+   local set and get).
+
+   VERY BIG NOTE: THIS DOES NOT ACTUALLY CHECK IF THIS IS THE
+   CORRECT L'. JUST SYNTHESIZES WHAT IT WOULD HAVE TO BE IF
+   IT IS CORRECT.
+
+ *)
+Definition synth_possible_resulting_local_ctx F (inst:instruction) (L:local_ctx) : (option local_ctx) + type_error :=
+  match inst with
+  | INop _ => inl (Some L)
+  | IUnreachable _ => inl None
+  | ICopy _
+  | IDrop _
+  | INum _ _
+  | INumConst _ _ => inl (Some L)
+  | IBlock _ L' _ => inl (Some L')
+  | ILoop _ _ => inl (Some L)
+  | IIte _ L' _ _ => inl (Some L')
+  | IBr _ _
+  | IReturn _ => inl None
+  | ILocalGet ψ i =>
+      match ψ with
+      | InstrT [] [τ] =>
+          match has_ref_flag_checker F τ NoRefs with
+          | inl () => inl (Some L)
+          | _ =>
+              match F.(fc_locals) !! i with
+              | Some ηs => inl (Some (<[ i := type_plug_prim ηs ]> L))
+              | _ => inr "NO"%string
+              end
+          end
+      | _ => inr "NO"%string
+      end
+  | ILocalSet ψ i =>
+      match ψ with
+      | InstrT [τ] [] => inl (Some (<[ i := τ ]> L))
+      | _ => inr "NO"%string
+      end
+  | ICodeRef _ _
+  | IInst _ _
+  | ICall _ _ _
+  | ICallIndirect _
+  | IInject _ _
+  | IInjectNew _ _ => inl (Some L)
+  | ICase _ L' _
+  | ICaseLoad _ _ L' _ => inl (Some L')
+  | IGroup _
+  | IUngroup _
+  | IFold _
+  | IUnfold _
+  | IPack _ => inl (Some L)
+  | IUnpack _ L' _ => inl (Some L')
+  | ITag _
+  | IUntag _
+  | ICast _
+  | INew _
+  | ILoad _ _ _
+  | IStore _ _
+  | ISwap _ _ => inl (Some L)
+  end.
+
+
+(* this is the old version with arity. just list_suffix is the same
+                let (e_n1, e_n2) := get_instruction_type_arity e_ψ in
+                let (es_n1, es_n2) := get_instruction_type_arity ψ in
+                if es_n1 <? e_n1
+                then INR "instruction has more arguments than large have_instruction type has"
+                else
+                  if es_n1 =? e_n1
+                  then (* equal arity case *)
+                    match e_ψ, ψ with
+                    | InstrT τs1_e τs2_e, InstrT τs1_es τs2_es =>
+                        if list_beq type type_beq τs1_e τs1_es
+                        then have_instruction_type_checker M F L_e es (InstrT τs2_e τs2_es) L'
+                        else INR "instruction arguments do not match large have_instruction arguments (exact case)"
+                    end
+                  else (* frame rule case *)
+                    match e_ψ, ψ with
+                    | InstrT τs1_e τs2_e, InstrT τs1_es τs2_es =>
+                        match list_suffix τs1_es τs1_e with (* ts1_es = ts_pref ++ ts1_e*)
+                        | Some τs_pref => have_instruction_type_checker M F L_e es (InstrT (τs_pref ++ τs2_e) τs2_es) L'
+                        | None => INR "can't frame out (multiple instructions)"
+                        end
+                    end *)
+
+Fixpoint unzip_sert (τs:list type) : option ((list kind) * (list type)) :=
+  match τs with
+  | [] => Some ([], [])
+  | τ :: τs =>
+      match τ with
+      | SerT k t =>
+          match unzip_sert τs with
+          | Some (ks, ts) => Some (k::ks, t::ts)
+          | None => None
+          end
+      | _ => None
+      end
+  end.
+
+Lemma unzip_sert_correct :
+  ∀ τs' κs τs, unzip_sert τs' = Some (κs, τs) -> τs' = zip_with SerT κs τs.
+Proof.
+  induction τs'.
+  - simpl. intros; inversion H. auto.
+  - intros. simpl in H. destruct a; try (by inversion H).
+    structural_auto. destruct p. clear H1.
+    inversion H. subst.
+    specialize (IHτs' l l0 eq_refl). subst.
+    auto.
+Qed.
+
+(* Will need a mutually recursive have_instruction_type too *)
+Fixpoint has_instruction_type_checker
+    (M:module_ctx) (F:function_ctx) (L:local_ctx)
+    (inst:instruction) (ψ:instruction_type) (L':local_ctx) {struct inst} : type_checker_res :=
+  let fix have_instruction_type_checker
+    (M:module_ctx) (F:function_ctx) (L:local_ctx)
+    (insts:list instruction) (ψ:instruction_type) (L':local_ctx) {struct insts} : type_checker_res :=
+    match insts with
+    | [] =>
+        if (local_ctx_beq L L')
+        then
+          match ψ with
+          | InstrT τs1 τs2 =>
+              if list_beq type type_beq τs1 τs2
+              then local_ctx_ok_checker F L
+              else INR "bad empty instructions type (not empties or frame)"
+          end
+        else INR "bad empty instructions type (local contexts don't match)"
+    | [e] =>
+        let e_ψ := proj_instr_ty e in
+        match has_instruction_type_checker M F L e e_ψ L' with
+        | inl () => (* now just to check if we need to frame stuff out *)
+            match e_ψ, ψ with
+            | InstrT τs1_e τs2_e, InstrT τs1_es τs2_es =>
+                match list_suffix τs1_es τs1_e, list_suffix τs2_es τs2_e with
+                | Some τs1_pref, Some τs2_pref =>
+                    (* ts1_es = ts1_pref ++ ts1_e, ts2_es = ts2_pref ++ ts2_e*)
+                    (* just need to check that ts1_pref = ts2_pref *)
+                    if list_beq type type_beq τs1_pref τs2_pref
+                    then ok_term
+                    else INR "can't frame out (single instruction)"
+                | _, _ => INR "inner instruction type doesn't match"
+                end
+            end
+        | err => err
+        end
+    | e :: es =>
+        let e_ψ := proj_instr_ty e in
+        match synth_possible_resulting_local_ctx F e L with
+        | inr _ => INR "this is either local get/set that is bad, so error?"
+        | inl None => INR "the type checker does not support break/return/unreachable in the middle of a block"
+        | inl (Some L_e) =>
+            match has_instruction_type_checker M F L e e_ψ L_e with
+            | inl () =>                 match e_ψ, ψ with
+                | InstrT τs1_e τs2_e, InstrT τs1_es τs2_es =>
+                    match list_suffix τs1_es τs1_e with (* τs1_es = τs_pref ++ τs1_es *)
+                    | Some τs_pref => have_instruction_type_checker M F L_e es (InstrT (τs_pref ++ τs2_e) τs2_es) L'
+                    | None => INR "instruction has more arguments than large have_instruction type has, or can't frame out"
+                    end
+                end
+            | err => err
+            end
+        end
+    end
+  in
+
+  match inst with
+  (*  BASE CASES  *)
+  | INop ψ_inner =>
+      if andb (andb (instruction_type_beq ψ (InstrT [] []))
+           (instruction_type_beq ψ_inner (InstrT [] []))) (local_ctx_beq L L')
+      then has_instruction_type_ok_checker F ψ L
+      else INR "incorrect instruction type for nop"
+  | IUnreachable ψ_inner =>
+      if instruction_type_beq ψ ψ_inner
+      then has_instruction_type_ok_checker F ψ L'
+      else INR "incorrect instruction type for unreachable"
+  | ICopy ψ_inner =>
+      if andb (instruction_type_beq ψ ψ_inner) (local_ctx_beq L L')
+      then
+        match ψ with
+        | InstrT [τ] [τ1;τ2] =>
+            if andb (type_beq τ τ1) (type_beq τ1 τ2)
+            then
+              match has_ref_flag_checker F τ GCRefs with
+              | inl () => has_instruction_type_ok_checker F ψ L
+              | _ => INR "incorrect copyability for instruction type for copy"
+              end
+            else INR "incorrect instruction type for copy"
+        | _ => INR "incorrect instruction type for copy"
+        end
+      else INR "incorrect instruction type for copy"
+  | IDrop ψ_inner =>
+      if andb (instruction_type_beq ψ ψ_inner) (local_ctx_beq L L')
+      then
+        match ψ with
+        | InstrT [τ] [] => has_instruction_type_ok_checker F ψ L
+        | _ => INR "incorrect instruction type for drop"
+        end
+      else INR "incorrect instruction type for drop"
+  | INum ψ_inner e =>
+      if andb (instruction_type_beq ψ ψ_inner) (local_ctx_beq L L')
+      then
+        match has_instruction_type_num_checker e ψ with
+        | inl () => has_instruction_type_ok_checker F ψ L
+        | err => err
+        end
+      else INR "incorrect instruction type for num"
+  | INumConst ψ_inner n =>
+      if andb (instruction_type_beq ψ ψ_inner) (local_ctx_beq L L')
+      then
+        match ψ with
+        | InstrT [] [τ] =>
+            if has_num_type_type τ
+            then has_instruction_type_ok_checker F ψ L
+            else INR "incorrect instruction type for numconst"
+        | _ => INR "incorrect instruction type for numconst"
+        end
+      else INR "incorrect instruction type for numconst"
+  (* not base cases lmao *)
+  | IBlock ψ_inner L_inner es =>
+      if andb (instruction_type_beq ψ ψ_inner) (local_ctx_beq L' L_inner)
+      then (* this INCORRECT but just to check if the recursion goes through *)
+        match ψ with
+        | InstrT τs1 τs2 =>
+            match have_instruction_type_checker M (F <| fc_labels ::= cons (τs2, L') |>) L es ψ L' with
+            | inl () => has_instruction_type_ok_checker F ψ L'
+            | err => err
+            end
+        end
+      else INR "incorrect instruction type for block"
+  | ILoop ψ_inner es =>
+      if andb (instruction_type_beq ψ ψ_inner) (local_ctx_beq L L')
+      then
+        match ψ with
+        | InstrT τs1 τs2 =>
+            match have_instruction_type_checker M (F <| fc_labels ::= cons (τs1, L) |>) L es ψ L with
+            | inl () => has_instruction_type_ok_checker F ψ L
+            | err => err
+            end
+        end
+      else INR "incorrect instruction type for loop"
+  | IIte ψ_inner L_inner es1 es2 =>
+      if andb (instruction_type_beq ψ ψ_inner) (local_ctx_beq L_inner L')
+      then
+        match ψ with
+        | InstrT τs1_full τs2 =>
+            match split_list_all_last τs1_full with
+            | Some (τs1, τ) =>
+                if type_beq τ type_i32
+                then
+                  match have_instruction_type_checker M (F <| fc_labels ::= cons (τs2, L') |>) L
+                          es1 (InstrT τs1 τs2) L' with
+                  | inl () =>
+                      match have_instruction_type_checker M (F <| fc_labels ::= cons (τs2, L') |>) L
+                          es2 (InstrT τs1 τs2) L' with
+                      | inl () => has_instruction_type_ok_checker F ψ L'
+                      | err => err
+                      end
+                  | err => err
+                  end
+                else INR "instruction type for ite does not have i32"
+            | None => INR "instruction type for ite does not have i32"
+            end
+        end
+      else INR "incorrect instruction type for ite"
+  | IBr ψ_inner i =>
+      if instruction_type_beq ψ ψ_inner
+      then
+        match F.(fc_labels) !! i with
+        | Some (τs, L_inner) =>
+            if local_ctx_beq L_inner L
+            then (* okay now we have to ensure ts1_full is split correctly *)
+              match ψ with
+              | InstrT τs1_full τs2 =>
+                  match list_suffix τs1_full τs with
+                  | Some τs1 =>
+                      if true (* if all ImDrop TODO *)
+                      then has_instruction_type_ok_checker F ψ L'
+                      else INR "incorrect instruction type for br"
+                  | None => INR "incorrect instruction type for br"
+                  end
+              end
+            else INR "incorrect instruction type for br"
+        | None => INR "incorrect instruction type for br, something with fc labels"
+        end
+      else INR "incorrect instruction type for br"
+  | IReturn ψ_inner =>
+      if instruction_type_beq ψ ψ_inner
+      then
+        let τs := F.(fc_return) in
+        match ψ with
+        | InstrT τs1_full τs2 =>
+            match list_suffix τs1_full τs with
+            | Some τs1 =>
+                if true (* if all ImDrop TODO *)
+                then has_instruction_type_ok_checker F ψ L'
+                else INR "incorrect instruction type for return"
+            | None => INR "incorrect instruction type for return"
+            end
+        end
+      else INR "incorrect instruction type for return"
+  | ILocalGet ψ_inner i => (* note this is for both TLocalGetMove and TLocalGetCopy *)
+      if andb (instruction_type_beq ψ ψ_inner) (true)
+      then
+        match L !! i with
+        | Some τ =>
+            match ψ with
+            | InstrT [] [τ'] =>
+                if type_beq τ τ'
+                then
+                  match has_ref_flag_checker F τ NoRefs with (* decision point *)
+                  | inl () =>
+                      if local_ctx_beq L L'
+                      then has_instruction_type_ok_checker F ψ L
+                      else INR "incorrect instruction type for local get"
+                  | inr _ =>
+                      match F.(fc_locals) !! i with
+                      | Some ηs =>
+                          if local_ctx_beq L' (<[ i := type_plug_prim ηs ]> L)
+                          then has_instruction_type_ok_checker F ψ L'
+                          else INR "incorrect instruction type for local get"
+                      | None => INR "incorrect instruction type for local get"
+                      end
+                  end
+                else INR "incorrect instruction type for local get"
+            | InstrT _ _ => INR "incorrect instruction type for local get (shape not [] -> [τ])"
+            end
+        | None => INR "incorrect instruction type for local get (i not in local context)"
+        end
+      else INR "incorrect instruction type for local get"
+  | ILocalSet ψ_inner i =>
+      if instruction_type_beq ψ ψ_inner
+      then
+        match L !! i with
+        | Some τ0 =>
+            match has_ref_flag_checker F τ0 NoRefs with
+            | inl () =>
+                match ψ with
+                | InstrT [τ] [] =>
+                    let L' := <[ i := τ ]> L in
+                    has_instruction_type_ok_checker F ψ L'
+                | _ => INR "incorrect instruction type for local set (shape not [τ] -> [])"
+                end
+            | err => err
+            end
+        | None => INR "bad instruction type for local set (not enough locals)"
+        end
+      else INR "incorrection instruction type for local set"
+  | ICodeRef ψ_inner i =>
+      if andb (instruction_type_beq ψ ψ_inner) (local_ctx_beq L L')
+      then
+        match ψ with
+        | InstrT [] [τ'] =>
+            match M.(mc_table) !! i with
+            | Some ϕ =>
+                if type_beq τ' (CodeRefT (VALTYPE (AtomR I32R) NoRefs) ϕ)
+                then has_instruction_type_ok_checker F ψ L
+                else INR "incorrect instruction type for coderef"
+            | None => INR "incorrect instruction type for coderef"
+            end
+        | InstrT _ _ => INR "incorrect instruction type for coderef (wrong shape)"
+        end
+      else INR "incorrect instruction type for coderef"
+  | IInst ψ_inner ix =>
+      if andb (instruction_type_beq ψ ψ_inner) (local_ctx_beq L L')
+      then
+        match ψ with
+        | InstrT [a] [b] =>
+            match a, b with
+            | CodeRefT κ ϕ, CodeRefT κ' ϕ' =>
+                if andb (kind_beq κ (VALTYPE (AtomR I32R) NoRefs)) (kind_beq κ κ')
+                then
+                  match function_type_inst_checker F ix ϕ ϕ' with
+                  | inl () => has_instruction_type_ok_checker F ψ L
+                  | err => err
+                  end
+                else INR "incorrect instruction type for IInst"
+            | _, _ => INR "incorrect instruction type for IINst"
+            end
+        | _ => INR "incorrect instruction type for IInst (wrong shape)"
+        end
+      else INR "incorrect instruction type for IINst"
+  | ICall ψ_inner i ixs =>
+      if andb (instruction_type_beq ψ ψ_inner) (local_ctx_beq L L')
+      then
+        match ψ with
+        | InstrT τs1 τs2 =>
+            match M.(mc_functions) !! i with
+            | Some ϕ =>
+                match function_type_insts_checker F ixs ϕ (MonoFunT τs1 τs2) with
+                | inl () => has_instruction_type_ok_checker F ψ L
+                | err => err
+                end
+            | None => INR "incorrect instruction type for call"
+            end
+        end
+      else INR "incorrect instruction type for call"
+  | ICallIndirect ψ_inner =>
+      if andb (instruction_type_beq ψ ψ_inner) (local_ctx_beq L L')
+      then
+        match ψ with
+        | InstrT τs1_full τs2 =>
+            match split_list_all_last τs1_full with
+            | Some (τs1, τ) =>
+                if type_beq τ (CodeRefT (VALTYPE (AtomR I32R) NoRefs) (MonoFunT τs1 τs2))
+                then has_instruction_type_ok_checker F ψ L
+                else INR "incorrect instruction type for call indirect"
+            | None => INR "incorrect instruction type for call indirect"
+            end
+        end
+      else INR "incorrect instruction type for call indirect"
+  | IInject ψ_inner i =>
+      if andb (instruction_type_beq ψ ψ_inner) (local_ctx_beq L L')
+      then
+        match ψ with
+        | InstrT [τ'] [a] =>
+            match a with
+            | SumT κ τs =>
+                match τs !! i with
+                | Some τ =>
+                    if type_beq τ' τ
+                    then has_instruction_type_ok_checker F ψ L
+                    else INR "incorrect instruction type for inject"
+                | None => INR "incorrect instruction type for inject"
+                end
+            | _ => INR "incorrect instruction type for inject (wrong shape)"
+            end
+        | _ => INR "incorrect instruction type for inject (wrong shape)"
+        end
+      else INR "incorrect instruction type for inject"
+  | IInjectNew ψ_inner i =>
+      if andb (instruction_type_beq ψ ψ_inner) (local_ctx_beq L L')
+      then
+        match ψ with
+        | InstrT [τ] [ref] =>
+            match ref with
+            | RefT κr μ (VariantT κv τs') =>
+                match unzip_sert τs' with
+                | Some (κs, τs) =>
+                    match τs !! i with
+                    | Some τ' =>
+                        if type_beq τ τ'
+                        then
+                          match mono_mem_checker μ with
+                          | inl () => has_instruction_type_ok_checker F ψ L
+                          | err => err
+                          end
+                        else INR "incorrect instruction type for inject new (not matching injections?)"
+                    | None => INR "incorrect instruction type for inject new (i out of bounds)"
+                    end
+                | None => INR "incorrect instruction type for inject new (variant is not all sered or smthn)"
+                end
+            | _ => INR "inocrrect instruction type for inject new (result isn't proper ref shape)"
+            end
+        | _ => INR "inocrrect instruction type for inject new (wrong shape)"
+        end
+      else INR "incorrect instruction type for inject new"
+  | ICase ψ_inner L_inner ess => INR "incomplete"
+  | ICaseLoad ψ_inner cm L_inner ess => INR "incomplete"
+  | IGroup ψ_inner =>
+      if andb (instruction_type_beq ψ ψ_inner) (local_ctx_beq L L')
+      then
+        match ψ with
+        | InstrT τs [a] =>
+            match a with
+            | ProdT κ τs' =>
+                if list_beq type type_beq τs τs'
+                then has_instruction_type_ok_checker F ψ L
+                else INR "incorrect instruction type for group"
+            | _ => INR "incorrect instruction type for group (wrong shape)"
+            end
+        | _ => INR "incorrect instruction type for group (wrong shape)"
+        end
+      else INR "incorrect instruction type for group"
+  | IUngroup ψ_inner =>
+      if andb (instruction_type_beq ψ ψ_inner) (local_ctx_beq L L')
+      then
+        match ψ with
+        | InstrT [a] τs =>
+            match a with
+            | ProdT κ τs' =>
+                if list_beq type type_beq τs τs'
+                then has_instruction_type_ok_checker F ψ L
+                else INR "incorrect instruction type for ungroup"
+            | _ => INR "incorrect instruction type for ungroup (wrong shape)"
+            end
+        | _ => INR "incorrect instruction type for ungroup (wrong shape)"
+        end
+      else INR "incorrect instruction type for ungroup"
+  | IFold ψ_inner =>
+      if andb (instruction_type_beq ψ ψ_inner) (local_ctx_beq L L')
+      then
+        match ψ with
+        | InstrT [τ0] [a] =>
+            match a with
+            | RecT κ τ =>
+                if type_beq τ0 (subst_type VarM VarR VarS (unscoped.scons (RecT κ τ) VarT) τ)
+                then has_instruction_type_ok_checker F ψ L
+                else INR "incorrect instruction type for fold"
+            | _ => INR "incorrect instruction type for fold (wrong shape)"
+            end
+        | _ => INR "incorrect instruction type for fold (wrong shape)"
+        end
+      else INR "incorrect instruction type for fold"
+  | IUnfold ψ_inner =>
+      if andb (instruction_type_beq ψ ψ_inner) (local_ctx_beq L L')
+      then
+        match ψ with
+        | InstrT [a] [τ0] =>
+            match a with
+            | RecT κ τ =>
+                if type_beq τ0 (subst_type VarM VarR VarS (unscoped.scons (RecT κ τ) VarT) τ)
+                then has_instruction_type_ok_checker F ψ L
+                else INR "incorrect instruction type for unfold"
+            | _ => INR "incorrect instruction type for unfold (wrong shape)"
+            end
+        | _ => INR "incorrect instruction type for unfold (wrong shape)"
+        end
+      else INR "incorrect instruction type for unfold"
+  | IPack ψ_inner =>
+      if andb (instruction_type_beq ψ ψ_inner) (local_ctx_beq L L')
+      then
+        match ψ with
+        | InstrT [τ] [τ'] =>
+            match packed_existential_checker F τ τ' with
+            | inl () => has_instruction_type_ok_checker F ψ L
+            | err => err
+            end
+        | _ => INR "incorrect instruction type for pack"
+        end
+      else INR "incorrect instruction type for pack"
+  | IUnpack ψ_inner L_inner es => INR "incomplete"
+  | ITag ψ_inner =>
+      if andb (instruction_type_beq ψ ψ_inner) (local_ctx_beq L L')
+      then
+        match ψ with
+        | InstrT [a] [b] =>
+            if andb (type_beq a type_i32) (type_beq b type_i31)
+            then has_instruction_type_ok_checker F ψ L
+            else INR "incorrect instruction type for tag"
+        | _ => INR "incorrect instruction type for tag (wrong shape)"
+        end
+      else INR "incorrect instruction type for tag"
+  | IUntag ψ_inner =>
+      if andb (instruction_type_beq ψ ψ_inner) (local_ctx_beq L L')
+      then
+        match ψ with
+        | InstrT [b] [a] =>
+            if andb (type_beq a type_i32) (type_beq b type_i31)
+            then has_instruction_type_ok_checker F ψ L
+            else INR "incorrect instruction type for untag"
+        | _ => INR "incorrect instruction type for untag (wrong shape)"
+        end
+      else INR "incorrect instruction type for untag"
+  | ICast ψ_inner =>
+      if andb (instruction_type_beq ψ ψ_inner) (local_ctx_beq L L')
+      then
+        match ψ with
+        | InstrT [τ] [τ'] =>
+            match type_eq_checker F τ τ' with
+            | inl () => has_instruction_type_ok_checker F ψ L
+            | err => err
+            end
+        | _ => INR "incorrect instruction type for cast (wrong shape)"
+        end
+      else INR "incorrect instruction type for cast"
+  | INew ψ_inner =>
+      if andb (instruction_type_beq ψ ψ_inner) (local_ctx_beq L L')
+      then
+        match ψ with
+        | InstrT [τ] [a] =>
+            match a with
+            | RefT κ μ (SerT κser τ') =>
+                if type_beq τ τ'
+                then
+                  match mono_mem_checker μ with
+                  | inl () => has_instruction_type_ok_checker F ψ L
+                  | err => err
+                  end
+                else INR "incorrect instruction type for new"
+            | _ => INR "incorrect instruction type for new (wrong shape)"
+            end
+        | _ => INR "incorrect instruction type for new (wrong shape)"
+        end
+      else INR "incorrect instruction type for new"
+  | ILoad ψ_inner π cm => (* note this will be both TLoadCopy and TLoadMove *)
+      INR "incomplete"
+  | IStore ψ_inner π => (* note this will be both TStoreWeak and TStoreStrong *)
+      if andb (instruction_type_beq ψ ψ_inner) (local_ctx_beq L L')
+      then
+        match ψ with
+        | InstrT [reft1; τval] [reft2] =>
+            if type_beq reft1 reft2 (* true = store weak *) (* false = store strong *)
+            then (* store weak *)
+              match reft1 with
+              | RefT κ μ τ =>
+                  match synth_resolving_path τ π None with
+                  | Some pr =>
+                      match has_ref_flag_checker F pr.(pr_target) GCRefs with
+                      | inl () =>
+                          match pr.(pr_target) with
+                          | SerT κser τval_inner =>
+                              if type_beq τval τval_inner
+                              then
+                                if (foldr (λ t:type, andb (check_ok_output (has_mono_size_checker F t))) true (pr.(pr_prefix)))
+                                then has_instruction_type_ok_checker F ψ L
+                                else INR "incorrect instruction type for weak store (prefix not all mono size)"
+                              else INR "incorrect instruction type for weak store (target ser bad inner type)"
+                          | _ => INR "inocrrect instruction type for weak store (target not ser)"
+                          end
+                      | err => err
+                      end
+                  | None => INR "incorrect instruction type for weak store (can't synth path)"
+                  end
+              | _ => INR "incorrect instruction type for weak store (not ref type)"
+              end
+            else (* store strong. Note: SerT kser tval = pr.(pr_replaced) *)
+              match reft1 with (* doing this in steps for automation. Might not help anyway lol *)
+              | RefT κ (BaseM MemMM) τ =>
+                  match reft2 with
+                  | RefT κ' (BaseM MemMM) prreplaced =>
+                      if true
+                      then (* we can finally start doing things omg *)
+                        match synth_resolving_with_outer_replaced τ π prreplaced τval  with
+                        | Some (pr, κser) =>
+                            match has_ref_flag_checker F pr.(pr_target) GCRefs with
+                            | inl () =>
+                                match grab_size F pr.(pr_target) with
+                                | Some σ =>
+                                    match grab_rep F τval with
+                                    | Some ρ =>
+                                        match eval_size EmptyEnv σ, eval_rep_size EmptyEnv ρ with
+                                        | Some n1, Some n2 =>
+                                            if andb (n1 =? n2) (foldr (λ t:type, andb (check_ok_output (has_mono_size_checker F t))) true (pr.(pr_prefix)))
+                                            then has_instruction_type_ok_checker F ψ L
+                                            else INR "incorrect instruction type for strong store (prefix not all mono size)"
+                                        | _, _ => INR "inc instr type for strong store (unmatching sizes)"
+                                        end
+                                    | None => INR "inc instr type for strong store"
+                                    end
+                                | None => INR "inc instr type for strong store"
+                                end
+                            | err => err
+                            end
+                        | None => INR "incorrect instruction type for strong store (can't synth path)"
+                        end
+                      else INR "incorrect instruction type for strong store (stored types don't match)"
+                  | _ => INR "inocrrect instruction type for strong store (second not ref with sert)"
+                  end
+              | _ => INR "incorrect instruction type for strong store (first not ref)"
+              end
+        | _ => INR "incorrect instruction type for store (wrong shape)"
+        end
+      else INR "incorrection instruction type for store (both types)"
+  | ISwap ψ_inner π =>
+      if andb (instruction_type_beq ψ ψ_inner) (local_ctx_beq L L')
+      then
+        match ψ with
+        | InstrT τs1 τs2 =>
+            if list_beq type type_beq τs1 τs2
+            then
+              match τs1 with (* note: doing this in multiple steps for automation purposes *)
+              | [reff; τval] =>
+                  match reff with
+                  | RefT κ μ τ =>
+                      match synth_resolving_path τ π None with
+                      | Some pr => (* now to match that pr has the right things *)
+                          match pr.(pr_target) with
+                          | SerT κser τval_inner =>
+                              if type_beq τval τval_inner
+                              then
+                                if (foldr (λ t:type, andb (check_ok_output (has_mono_size_checker F t))) true (pr.(pr_prefix)))
+                                then has_instruction_type_ok_checker F ψ L
+                                else INR "improper synthesized path target"
+                              else INR "improper synthesized path target"
+                          | _ => INR "improper synthesized path target"
+                          end
+                      | None => INR "couldn't synthesize path"
+                      end
+                  | _ => INR "bad instruction type for swap (first arg not ref)"
+                  end
+              | _ => INR "bad instruction type for swap (wrong shape)"
+              end
+            else INR "bad instruction type for swap"
+        end
+      else INR "incorrect instruction type for swap"
+  end.
+
+
+(* TODO at the end make sure this is a direct copy of above *)
+Fixpoint have_instruction_type_checker
+    (M:module_ctx) (F:function_ctx) (L:local_ctx)
+    (insts:list instruction) (ψ:instruction_type) (L':local_ctx) {struct insts} : type_checker_res :=
+    match insts with
+    | [] =>
+        if (local_ctx_beq L L')
+        then
+          match ψ with
+          | InstrT τs1 τs2 =>
+              if list_beq type type_beq τs1 τs2
+              then local_ctx_ok_checker F L
+              else INR "bad empty instructions type (not empties or frame)"
+          end
+        else INR "bad empty instructions type (local contexts don't match)"
+    | [e] =>
+        let e_ψ := proj_instr_ty e in
+        match has_instruction_type_checker M F L e e_ψ L' with
+        | inl () => (* now just to check if we need to frame stuff out *)
+            match e_ψ, ψ with
+            | InstrT τs1_e τs2_e, InstrT τs1_es τs2_es =>
+                match list_suffix τs1_es τs1_e, list_suffix τs2_es τs2_e with
+                | Some τs1_pref, Some τs2_pref =>
+                    (* ts1_es = ts1_pref ++ ts1_e, ts2_es = ts2_pref ++ ts2_e*)
+                    (* just need to check that ts1_pref = ts2_pref *)
+                    if list_beq type type_beq τs1_pref τs2_pref
+                    then ok_term
+                    else INR "can't frame out (single instruction)"
+                | _, _ => INR "inner instruction type doesn't match"
+                end
+            end
+        | err => err
+        end
+    | e :: es =>
+        let e_ψ := proj_instr_ty e in
+        match synth_possible_resulting_local_ctx F e L with
+        | inr _ => INR "this is either local get/set that is bad, so error?"
+        | inl None => INR "the instr we're processing is either uncreachable, break, or return, with more commands to follow. unsure how to deal with rn TODO"
+        | inl (Some L_e) =>
+            match has_instruction_type_checker M F L e e_ψ L_e with
+            | inl () =>                 match e_ψ, ψ with
+                | InstrT τs1_e τs2_e, InstrT τs1_es τs2_es =>
+                    match list_suffix τs1_es τs1_e with (* τs1_es = τs_pref ++ τs1_es *)
+                    | Some τs_pref => have_instruction_type_checker M F L_e es (InstrT (τs_pref ++ τs2_e) τs2_es) L'
+                    | None => INR "instruction has more arguments than large have_instruction type has, or can't frame out"
+                    end
+                end
+            | err => err
+            end
+        end
+    end.
+
+
+Ltac my_auto5 :=
+  try structural_auto; try boolean_equality_auto; try
+  match goal with
+  | H: (synth_resolving_path _ _ _ = Some _) |- _ => apply synth_resolving_path_correct in H; auto
+  | H: (synth_resolving_with_outer_replaced _ _ _ _ = Some (_, _)) |- _ => apply synth_resolving_with_outer_replaced_correct in H; auto
+  | H: (kind_ok_checker _ _ = inl ()) |- _ => apply kind_ok_checker_correct in H; auto
+  | H: (kind_ok_checker _ _ = ok_term) |- _ => apply kind_ok_checker_correct in H; auto
+  | H: (mem_ok_checker _ _ = inl ()) |- _ => apply mem_ok_checker_correct in H; auto
+  | H: (mem_ok_checker _ _ = ok_term) |- _ => apply mem_ok_checker_correct in H; auto
+  | H: (rep_ok_checker _ _ = inl ()) |- _ => apply rep_ok_checker_correct in H; auto
+  | H: (rep_ok_checker _ _ = ok_term) |- _ => apply rep_ok_checker_correct in H; auto
+  | H: (size_ok_checker _ _ = inl ()) |- _ => apply size_ok_checker_correct in H; auto
+  | H: (size_ok_checker _ _ = ok_term) |- _ => apply size_ok_checker_correct in H; auto
+  | H: (type_ok_checker _ _ = inl ()) |- _ => apply type_ok_checker_correct in H; auto
+  | H: (type_ok_checker _ _ = ok_term) |- _ => apply type_ok_checker_correct in H; auto
+  | H: (function_type_ok_checker _ _ = inl ()) |- _ => apply function_type_ok_checker_correct in H; auto
+  | H: (function_type_ok_checker _ _ = ok_term) |- _ => apply function_type_ok_checker_correct in H; auto
+  | H: (has_kind_checker _ _ _ = inl ()) |- _ => apply has_kind_checker_correct in H; auto
+  | H: (has_kind_checker _ _ _ = ok_term) |- _ => apply has_kind_checker_correct in H; auto
+  | H: (has_instruction_type_ok_checker _ _ _ = ok_term) |- _ => apply has_instruction_type_ok_checker_correct in H; auto
+  | H: (has_instruction_type_ok_checker _ _ _ = inl ()) |- _ => apply has_instruction_type_ok_checker_correct in H; auto
+  | H: (has_instruction_type_num_checker _ _ = ok_term) |- _ => apply has_instruction_type_num_checker_correct in H; auto
+  | H: (has_instruction_type_num_checker _ _ = inl ()) |- _ => apply has_instruction_type_num_checker_correct in H; auto
+  | H: (has_ref_flag_checker _ _ _ = ok_term) |- _ => apply has_ref_flag_checker_correct in H; auto
+  | H: (has_ref_flag_checker _ _ _ = inl ()) |- _ => apply has_ref_flag_checker_correct in H; auto
+  | H: (has_num_type_type _ = true) |- _ => apply has_num_type_type_correct in H; destruct H as [ν H]; subst; auto
+  | H: (check_if_subkind _ _ = inl ()) |- _ =>
+      try( by (eapply check_if_subkind_works_with_has_kind; try constructor; auto))
+  | H: (check_if_subkind _ _ = ok_term) |- _ =>
+      try( by (eapply check_if_subkind_works_with_has_kind; try constructor; auto))
+end.
+
+
+Lemma has_instruction_type_checker_correct :
+  ∀ M F L inst ψ L',
+    has_instruction_type_checker M F L inst ψ L' = ok_term ->
+    has_instruction_type M F L inst ψ L'.
+Proof.
+  intros.
+  Opaque have_instruction_type_checker.
+  induction inst; unfold has_instruction_type_checker in H.
+  1-5: repeat my_auto5; by constructor.
+  29: {
+    repeat my_auto5. apply (TSwap _ _ _ _ _ _ p k k0 _); auto. (* foldr lemma *)
+    admit.
+    }
+  28: {
+    structural_auto. clear H1. structural_auto. repeat boolean_equality_auto.
+    repeat my_auto5.
+    - clear H1 H2 H3 H4 H5 H6 H7 H8 H9 H10.
+      clear H12 H13.
+      apply (TStoreWeak _ _ _ _ _ _ _ p _ k0 ); auto; [rewrite HMatch; auto |].
+      (* foldr lemma *)
+      admit.
+    - clear H1 H2 H3 H4 H5 H6 H7 H8 H9 H10 H11 H12 H13 H14 H15 H16.
+      clear H18 H19 H20 H21.
+      apply Nat.eqb_eq in H0.
+      destruct HMatch12 as [Hres Htosub]; subst.
+
+      apply (TStoreStrong M F L' l t2 t0 p0 s r k k0 k1); auto.
+      (* some boring stuff *)
+      all: admit.
+  }
+  23-24: repeat my_auto5; by constructor.
+  - admit.
+Admitted.
+
+
+Lemma have_instruction_type_checker_correct :
+  ∀ M F L insts ψ L',
+    have_instruction_type_checker M F L insts ψ L' = ok_term ->
+    have_instruction_type M F L insts ψ L'.
+Proof. Admitted.
+
+Fixpoint synth_possible_resulting_local_ctx_insts F insts L : (option local_ctx) + type_error :=
+  match insts with
+  | [] => inl (Some L)
+  | [i] =>
+      match synth_possible_resulting_local_ctx F i L with
+      | inl (Some L') => inl (Some L')
+      | inl (None) => inl (Some L) (* IF LAST INSTR IS BREAK/RETURN, JUST KEEP SAME LOCAL CTX *)
+      | inr a => inr a
+      end
+  | i :: rest =>
+      match synth_possible_resulting_local_ctx F i L with
+      | inl (Some L') => synth_possible_resulting_local_ctx_insts F rest L'
+      | inl (None) => inl (None) (* IF BREAK/RETURN IN THE MIDDLE, FAIL *)
+      | inr a => inr a
+      end
+  end.
+
+Definition has_function_type_checker
+    (M:module_ctx) (mf:module_function) (ft:function_type) : type_checker_res :=
+  if function_type_beq mf.(mf_type) ft
+  then
+    let ϕ := flatten_function_type mf.(mf_type) in
+    let K := kc_of_fft ϕ in
+    match mapM (eval_rep_prim EmptyEnv) mf.(mf_locals) with
+    | Some ηss =>
+        let F := Build_function_ctx ϕ.(fft_out) ηss [] K ϕ.(fft_type_vars) in
+        let L := map type_plug_prim ηss in
+        let ψ := InstrT ϕ.(fft_in) ϕ.(fft_out) in
+        match synth_possible_resulting_local_ctx_insts F (mf.(mf_body)) L with
+        | inl (Some L') =>
+            if (foldr (λ t:type, andb (check_ok_output (has_ref_flag_checker F t NoRefs))) true L')
+            then have_instruction_type_checker M F L mf.(mf_body) ψ L'
+            else INR "bad"
+        | inl None => INR "don't know how to deal with breaks and stuff yet for synthing local ctx"
+        | inr a => INR "error in synthing local ctx (e.g. bad local get/set)"
+        end
+    | None => INR "can't give function type"
+    end
+  else INR "bad".
+Lemma has_function_type_checker_correct :
+  ∀ M mf ft, has_function_type_checker M mf ft = ok_term ->
+             has_function_type M mf ft.
+Proof.
+  intros.
+  Opaque have_instruction_type_checker.
+  unfold has_function_type_checker in H.
+  repeat my_auto5.
+  rename l into ηss. rename l0 into L'.
+  clear H1 H2 H3 H4 H5.
+  apply (TFunction M mf ηss L'); auto.
+  - admit. (* just a foldr lemma *)
+  - by apply have_instruction_type_checker_correct in H.
+Admitted.
+
+
+
+Definition has_module_type_checker (m:module) (mt:module_type) : type_checker_res :=
+  let ϕs := m.(m_imports) ++ map mf_type m.(m_functions) in
+  match nths_error ϕs m.(m_table) with
+  | Some table =>
+      match nths_error ϕs (map me_desc m.(m_exports)) with
+      | Some exports =>
+          if module_type_beq mt (Build_module_type m.(m_imports) exports)
+          then
+            let M := Build_module_ctx ϕs table in
+            if (foldr (λ mf, andb (check_ok_output (has_function_type_checker M mf mf.(mf_type))))
+                      true m.(m_functions))
+            then ok_term
+            else INR "function types don't equal"
+          else INR "suggested module type not equal to what it needs to be"
+      | None => INR "bad exports"
+      end
+  | None => INR "bad table"
+  end
+.
+Lemma has_module_type_checker_correct :
+  ∀ m mt, has_module_type_checker m mt = ok_term -> has_module_type m mt.
+Proof.
+  intros.
+  Opaque has_function_type_checker. Opaque module_type_beq.
+  unfold has_module_type_checker in H.
+  repeat my_auto5.
+  rename l into table.
+  rename l0 into exports.
+  apply (TModule m table exports); auto.
+  (* and this is just a foldr lemma *)
+
+Admitted.
+
+Definition synth_module_type (m:module) : option module_type :=
+  let ϕs := m.(m_imports) ++ map mf_type m.(m_functions) in
+      match nths_error ϕs (map me_desc m.(m_exports)) with
+      | Some exports =>
+          Some (Build_module_type m.(m_imports) exports)
+      | None => None
+      end.
+
+Definition has_module_type_checker_with_synth (m:module) : type_checker_res :=
+  match synth_module_type m with
+  | Some mt => has_module_type_checker m mt
+  | None => INR "couldn't synthesize module type"
+  end.
+
+(* rebasing went okay *)
